Switched Step 4 part 2 to use Game 5 invariant instead of Red_ROM invariant. Further simplifications made as well.

nsl/Games.ec
@@ -1,6 +1,9 @@
-(* Intermediate Games *)
 require import AllCore FMap FSet Distr NSL.
 import GWAKEc AEADc.
+
+(* ------------------------------------------------------------------------------------------ *)
+(* Intermediate Games *)
+(* ------------------------------------------------------------------------------------------ *)
 
 (* Inlining and removing psk from instance state *)
 module Game1 = {
@@ -104,13 +107,10 @@ module Game1 = {
       match st with
       | Accepted trace k' => {
         k <- k';
-        (* Get partners *)
         ps <- get_partners (a, i) (Some trace) role state_map;
         if (card ps <= 1) {
           ps <- get_observed_partners (a, i) state_map;
-          (* If we have no observed partners then, we can test *)
           if (card ps <> 0) {
-            (* If a partner has revealed something, we must use the same key *)
             p <- pick ps;
             (p_role, p_st) <- oget state_map.[p];
             if (p_st is Observed _ p_k) {
@@ -223,7 +223,7 @@ module Game4 = Game3 with {
 
 (* Delay nonce sampling *)
 module Game5 = Game4 with {
-  var prfkey_map : (ctxt, nonce * nonce) fmap
+  var prfkey_map : (msg_data * ctxt, nonce * nonce) fmap
   
   proc init_mem [
     -1 + { prfkey_map <- empty; }
@@ -250,14 +250,14 @@ module Game5 = Game4 with {
     },
     ^if.^match#IPending.^match#Some.^if.^skey<- ~ { 
       (na, ok) <$ dnonce `*` dnonce;
-      prfkey_map.[caf] <- (na, ok);
+      prfkey_map.[(msg3_data a b ca m2, caf)] <- (na, ok);
       skey <- prf (na, ok) (a, b);
     } 
   ]
 
   proc send_fin [
     ^if.^match#RPending.^match#Some.^skey<- ~ {
-      skey <- prf (oget prfkey_map.[m3]) (a, b);
+      skey <- prf (oget prfkey_map.[(msg3_data a b ca cb, m3)]) (a, b);
     }
   ]
 }.
@@ -311,29 +311,24 @@ GWAKE0_inv sm psk c j =>
 GWAKE0_inv sm.[(a, i) <- v] psk c j.
 proof.
 move=> neq
-[ 
-| r 
-| b na c1 kab
-| b na nb c1 c2 kba
-| r tr k
-| r tr k
+[
+smbj
+| r smbj
+| b na c1 kab smbj pskcb
+| b na nb c1 c2 kba smbj pskcb
+| r tr k smbj
+| r tr k smbj
 ].
-+ move=> smbj.
-  apply GWAKE0_undef.
++ apply GWAKE0_undef.
   by rewrite get_set_neqE.
-+ move=> smbj.
-  apply (GWAKE0_aborted _ _ _ _ r).
++ apply (GWAKE0_aborted _ _ _ _ r).
   by rewrite get_set_neqE.
-+ move=> smbj pskcb.
-  apply (GWAKE0_ipending _ _ _ _ b na c1 kab) => //.
++ apply (GWAKE0_ipending _ _ _ _ b na c1 kab) => //.
   by rewrite get_set_neqE.
-+ move=> smbj pskcb.
-  apply (GWAKE0_rpending _ _ _ _ b na nb c1 c2 kba)=> //.
++ apply (GWAKE0_rpending _ _ _ _ b na nb c1 c2 kba)=> //.
   by rewrite get_set_neqE.
-+ move=> smbj.
-  apply (GWAKE0_accepted _ _ _ _ r tr k)=> //.
++ apply (GWAKE0_accepted _ _ _ _ r tr k)=> //.
   by rewrite get_set_neqE.
-move=> smbj.
 apply (GWAKE0_observed _ _ _ _ r tr k)=> //.
 by rewrite get_set_neqE.
 qed.
@@ -346,37 +341,47 @@ proof.
 proc; inline *.
 if => //.
 auto => />.
-move => &m inv1 inv3 k _ a' i'.
-case: (inv1 a' i'). 
-+ move=> sm.
-  by apply GWAKE0_undef.
-+ move => r sm.
-  exact (GWAKE0_aborted _ _ _ _ r).
-+ move => b na c1 kab sm psk.
-  apply (GWAKE0_ipending _ _ _ _ b na c1 kab) => //.
+move => &m inv abnin pk _ a' i'.
+case: (inv a' i') =>
+[ 
+smbj
+| r smbj
+| b na c1 kab smbj pskcb
+| b na nb c1 c2 kba smbj pskcb
+| r tr k smbj
+| r tr k smbj
+].
++ exact GWAKE0_undef.
++ exact (GWAKE0_aborted _ _ _ _ r).
++ apply (GWAKE0_ipending _ _ _ _ b na c1 kab) => //.
+  smt(get_setE).  
++ apply (GWAKE0_rpending _ _ _ _ b na nb c1 c2 kba) => //.
   smt(get_setE).
-+ move => b na nb c1 c2 kba sm psk.
-  apply (GWAKE0_rpending _ _ _ _ b na nb c1 c2 kba) => //.
-  smt(get_setE).
-+ move => r tr k'.
-  exact (GWAKE0_accepted _ _ _ _ r tr k').
-move => r tr k'.
-exact (GWAKE0_observed _ _ _ _ r tr k').
++ exact (GWAKE0_accepted _ _ _ _ r tr k).
+exact (GWAKE0_observed _ _ _ _ r tr k).
 qed.
     
+lemma GWAKE0_inv_aborted a i b j r sm pm: GWAKE0_inv sm pm a i => GWAKE0_inv sm.[(b, j) <- (r, Aborted)] pm a i.
+proof.
+move=> inv.
+case ((a, i) = (b, j)) => /> => [|neq_ai].
+- apply (GWAKE0_aborted _ _ _ _ r).
+  by rewrite get_set_sameE.
+exact /GWAKE0_inv_neq/inv.
+qed.
+
 hoare GWAKE0_inv_send_msg1: GWAKE0(NSL).send_msg1:
     (forall a i, GWAKE0_inv GWAKEb.state_map GWAKEb.psk_map a i)
 ==> 
     (forall a i, GWAKE0_inv GWAKEb.state_map GWAKEb.psk_map a i).
 proc; inline *.
 sp; if => //.
-auto => /> &m inv ainin abin na _ ca _ a' i'.
+auto => /> &m inv ainin /domE abin na _ ca _ a' i'.
 case ((a', i') = (a, i){m}) => /> => [|neq_ai].
 + apply (GWAKE0_ipending _ _ _ _ b{m} na ca (oget GWAKEb.psk_map.[(a, b)]{m})).
   - by rewrite get_set_sameE.
-  smt().
-apply GWAKE0_inv_neq => //.
-exact inv.
+  exact some_oget.
+exact /GWAKE0_inv_neq/inv.
 qed.
     
 hoare GWAKE0_inv_send_msg2: GWAKE0(NSL).send_msg2:
@@ -387,21 +392,17 @@ proof.
 proc; inline *.
 sp; if => //.
 sp; match.
-+ match None 2; 1: by auto.
++ match None ^match; 1: by auto.
   auto => /> &m decn st inv bjnin abin a' i'.
-  case ((a', i') = (b, j){m}) => /> => [|neq_ai].
-  - apply (GWAKE0_aborted _ _ _ _ Responder). smt(get_setE).
-  apply GWAKE0_inv_neq => //.
-  exact inv.
-match Some 5; 1: auto => /#.
-auto => /> &m decn st inv bjnin abin n _ cb0 cin a' i'.
-case ((a', i') = (b, j){m}) => [eq_ai|neq_ai].
+  exact /GWAKE0_inv_aborted/inv.
+match Some ^match; 1: by auto=> /#.
+auto => /> &m decn st inv bjnin /domE abin n _ cb0 cin a' i'.
+case ((a', i') = (b, j){m}) => /> => [|neq_ai].
 + rewrite /get_as_Some //=.
   apply (GWAKE0_rpending _ _ _ _ a0{m} na{m} n ca{m} cb0 (oget GWAKEb.psk_map.[(a0, b)]{m})).
-  - by rewrite get_setE eq_ai //=. 
-  smt().
-apply GWAKE0_inv_neq => //.
-exact inv.
+  - by rewrite get_set_sameE.
+  exact some_oget.
+exact /GWAKE0_inv_neq/inv.
 qed.
 
 hoare GWAKE0_inv_send_msg3: GWAKE0(NSL).send_msg3:
@@ -411,22 +412,18 @@ hoare GWAKE0_inv_send_msg3: GWAKE0(NSL).send_msg3:
 proof.
 proc; inline *.
 sp; if => //.
-sp; match; 2..5: auto.
+sp; match; 2..5: by auto.
 sp; match.
-- match None 2; 1: by auto.
+- match None ^match; 1: by auto.
   auto => /> &m decn st inv aiin a' i'.
-  case ((a', i') = (a, i){m}) => /> => [|neq_ai].
-  - apply (GWAKE0_aborted _ _ _ _ Initiator). smt(get_setE).
-  apply GWAKE0_inv_neq => //.
-  exact inv.
-match Some 6; 1: auto => /#.
+  exact /GWAKE0_inv_aborted/inv.
+match Some ^match; 1: auto => /#.
 auto => /> &m decn st inv aiin n _ ca0 cin a' i'.
-case ((a', i') = (a, i){m}) => [eq_ai|neq_ai].
+case ((a', i') = (a, i){m}) => /> => [|neq_ai].
 + rewrite /get_as_Some //=.
   apply (GWAKE0_accepted _ _ _ _ Initiator (m1{m}, m2{m}, ca0) (prf (na{m}, nb{m}) (a{m}, b{m}))).
-  - by rewrite get_setE eq_ai //=. 
-apply GWAKE0_inv_neq => //.
-exact inv.
+  by rewrite get_set_sameE.
+exact /GWAKE0_inv_neq/inv.
 qed.
 
 hoare GWAKE0_inv_send_fin: GWAKE0(NSL).send_fin:
@@ -436,22 +433,18 @@ hoare GWAKE0_inv_send_fin: GWAKE0(NSL).send_fin:
 proof.
 proc; inline *.
 sp; if => //.
-sp; match; 1: auto; 2..4: auto.
+sp; match; 1, 3..5: by auto.
 sp; match.
-- match None 2; 1: by auto.
+- match None ^match; 1: by auto.
   auto => /> &m decn st inv bjin a' i'.
-  case ((a', i') = (b, j){m}) => /> => [|neq_ai].
-  - apply (GWAKE0_aborted _ _ _ _ Responder). smt(get_setE).
-  apply GWAKE0_inv_neq => //.
-  exact inv.
-match Some 4; 1: auto => /#.
+  exact /GWAKE0_inv_aborted/inv.
+match Some ^match; 1: auto => /#.
 auto => /> &m decn st inv bjin a' i'.
-case ((a', i') = (b, j){m}) => [eq_ai|neq_ai].
+case ((a', i') = (b, j){m}) => /> => [|neq_ai].
 + rewrite /get_as_Some //=.
   apply (GWAKE0_accepted _ _ _ _ Responder (m1{m}, m2{m}, m3{m}) (prf (na{m}, nb{m}) (a{m}, b{m}))).
-  - by rewrite get_setE eq_ai //=. 
-apply GWAKE0_inv_neq => //.
-exact inv.
+  by rewrite get_set_sameE. 
+exact /GWAKE0_inv_neq/inv.
 qed.
 
 hoare GWAKE0_inv_rev_skey: GWAKE0(NSL).rev_skey:
@@ -461,16 +454,15 @@ hoare GWAKE0_inv_rev_skey: GWAKE0(NSL).rev_skey:
 proof.
 proc; inline *.
 sp; if => //.
-sp; match; 1..2: auto; 2..3: auto.
+sp; match; 1,2,4,5: by auto.
 sp; if => //.
 wp 2.
 conseq (: _ ==> true); last by auto.
 auto => /> &m st inv aiin _ k a' i'.
-case ((a', i') = (a, i){m}) => [eq_ai|neq_ai].
+case ((a', i') = (a, i){m}) => /> => [|neq_ai].
 - apply (GWAKE0_observed _ _ _ _ role{m} trace{m} k).
-  smt(get_setE).
-apply GWAKE0_inv_neq => //.
-exact inv.
+  by rewrite get_set_sameE.
+exact /GWAKE0_inv_neq/inv.
 qed.
 
 hoare GWAKE0_inv_test: GWAKE0(NSL).test:
@@ -480,16 +472,15 @@ hoare GWAKE0_inv_test: GWAKE0(NSL).test:
 proof.
 proc; inline *.
 sp; if => //.
-sp; match; 1..2: auto; 2..3: auto.
+sp; match; 1,2,4,5: by auto.
 sp; if => //.
 wp 2.
 conseq (: _ ==> true); last by auto.
 auto => /> &m st inv aiin _ k a' i'.
-case ((a', i') = (a, i){m}) => [eq_ai|neq_ai].
+case ((a', i') = (a, i){m}) => /> => [|neq_ai].
 - apply (GWAKE0_observed _ _ _ _ role{m} trace{m} k).
-  smt(get_setE).
-apply GWAKE0_inv_neq => //.
-exact inv.
+  by rewrite get_set_sameE.
+exact /GWAKE0_inv_neq/inv.
 qed.
 
 (* ------------------------------------------------------------------------------------------ *)
@@ -518,30 +509,34 @@ Game1_inv sm.[(a, i) <- v] psk c j.
 proof.
 move=> neq
 [ 
-| r 
-| b na c1 kab
-| b na nb c1 c2 kba
-| r tr k
-| r tr k
+smbj
+| r smbj
+| b na c1 kab smbj pskcb
+| b na nb c1 c2 kba smbj pskcb
+| r tr k smbj
+| r tr k smbj
 ].
-+ move=> smbj.
-  apply Game1_undef.
++ apply Game1_undef.
   by rewrite get_set_neqE.
-+ move=> smbj.
-  apply (Game1_aborted _ _ _ _ r).
++ apply (Game1_aborted _ _ _ _ r).
   by rewrite get_set_neqE.
-+ move=> smbj pskcb.
-  apply (Game1_ipending _ _ _ _ b na c1 kab) => //.
++ apply (Game1_ipending _ _ _ _ b na c1 kab) => //.
   by rewrite get_set_neqE.
-+ move=> smbj pskcb.
-  apply (Game1_rpending _ _ _ _ b na nb c1 c2 kba)=> //.
++ apply (Game1_rpending _ _ _ _ b na nb c1 c2 kba)=> //.
   by rewrite get_set_neqE.
-+ move=> smbj.
-  apply (Game1_accepted _ _ _ _ r tr k)=> //.
++ apply (Game1_accepted _ _ _ _ r tr k)=> //.
   by rewrite get_set_neqE.
-move=> smbj.
 apply (Game1_observed _ _ _ _ r tr k)=> //.
 by rewrite get_set_neqE.
+qed.
+
+lemma Game1_inv_aborted a i b j r sm pm: Game1_inv sm pm a i => Game1_inv sm.[(b, j) <- (r, Aborted)] pm a i.
+proof.
+move=> inv.
+case ((a, i) = (b, j)) => /> => [|neq_ai].
+- apply (Game1_aborted _ _ _ _ r).
+  by rewrite get_set_sameE.
+exact /Game1_inv_neq/inv.
 qed.
 
 hoare Game1_inv_gen_pskey: Game1.gen_pskey:
@@ -552,22 +547,24 @@ proof.
 proc; inline *.
 if => //.
 auto => />.
-move => &m inv1 inv3 k _ a' i'.
-case: (inv1 a' i'). 
-+ move=> sm.
-  by apply Game1_undef.
-+ move => r sm.
-  exact (Game1_aborted _ _ _ _ r).
-+ move => b na c1 kab sm psk.
-  apply (Game1_ipending _ _ _ _ b na c1 kab) => //.
-  smt(get_setE).
-+ move => b na nb c1 c2 kba sm psk.
-  apply (Game1_rpending _ _ _ _ b na nb c1 c2 kba) => //.
-  smt(get_setE).
-+ move => r tr k'.
-  exact (Game1_accepted _ _ _ _ r tr k').
-move => r tr k'.
-exact (Game1_observed _ _ _ _ r tr k').
+move => &m inv abnin pk _ a' i'.
+case: (inv a' i') =>
+[ 
+smbj
+| r smbj
+| b na c1 kab smbj pskcb
+| b na nb c1 c2 kba smbj pskcb
+| r tr k smbj
+| r tr k smbj
+].
++ exact Game1_undef.
++ exact (Game1_aborted _ _ _ _ r).
++ apply (Game1_ipending _ _ _ _ b na c1 kab) => //.
+  by rewrite mem_set pskcb.
++ apply (Game1_rpending _ _ _ _ b na nb c1 c2 kba) => //.
+  by rewrite mem_set pskcb.
++ exact (Game1_accepted _ _ _ _ r tr k).
+exact (Game1_observed _ _ _ _ r tr k).
 qed.
     
 hoare Game1_inv_send_msg1: Game1.send_msg1:
@@ -578,12 +575,10 @@ proof.
 proc; inline *.
 sp; if => //.
 auto => /> &m inv ainin abin na _ ca _ a' i'.
-case ((a', i') = (a, i){m}) => /> => [|neq_ai].
-+ apply (Game1_ipending _ _ _ _ b{m} na ca witness).
-  - by rewrite get_set_sameE.
-  smt().
-apply Game1_inv_neq => //.
-exact inv.
+case ((a', i') = (a, i){m}) => [[] <<- <-|neq_ai].
++ apply (Game1_ipending _ _ _ _ b{m} na ca witness)=> //.
+  by rewrite get_set_sameE.
+exact /Game1_inv_neq/inv.
 qed.
     
 hoare Game1_inv_send_msg2: Game1.send_msg2:
@@ -595,18 +590,13 @@ proc; inline *.
 sp; if => //.
 sp; match.
 + auto => /> &m decn st inv bjnin abin a' i'.
-  case ((a', i') = (b, j){m}) => /> => [|neq_ai].
-  - apply (Game1_aborted _ _ _ _ Responder). smt(get_setE).
-  apply Game1_inv_neq => //.
-  exact inv.
+  exact /Game1_inv_aborted/inv.
 auto => /> &m decn st inv bjnin abin n _ cb0 cin a' i'.
-case ((a', i') = (b, j){m}) => [eq_ai|neq_ai].
+case ((a', i') = (b, j){m}) => [[] <<- <-|neq_ai].
 + rewrite /get_as_Some //=.
-  apply (Game1_rpending _ _ _ _ a{m} na{m} n ca{m} cb0 witness).
-  - by rewrite get_setE eq_ai //=. 
-  smt().
-apply Game1_inv_neq => //.
-exact inv.
+  apply (Game1_rpending _ _ _ _ a{m} na{m} n ca{m} cb0 witness) => //.
+  by rewrite get_set_sameE.
+exact /Game1_inv_neq/inv.
 qed.
 
 hoare Game1_inv_send_msg3: Game1.send_msg3:
@@ -619,17 +609,13 @@ sp; if => //.
 sp; match; 2..5: auto.
 sp; match.
 + auto => /> &m decn st inv abin a' i'.
-  case ((a', i') = (a, i){m}) => /> => [|neq_ai].
-  - apply (Game1_aborted _ _ _ _ Initiator). smt(get_setE).
-  apply Game1_inv_neq => //.
-  exact inv.
+  exact /Game1_inv_aborted/inv.
 auto => /> &m decn st inv aiin n _ ca0 cin a' i'.
-case ((a', i') = (a, i){m}) => [eq_ai|neq_ai].
+case ((a', i') = (a, i){m}) => [<-|neq_ai].
 + rewrite /get_as_Some //=.
   apply (Game1_accepted _ _ _ _ Initiator (m1{m}, m2{m}, ca0) (prf (na{m}, nb{m}) (a{m}, b{m}))).
-  - by rewrite get_setE eq_ai //=. 
-apply Game1_inv_neq => //.
-exact inv.
+  by rewrite get_set_sameE.
+exact /Game1_inv_neq/inv.
 qed.
 
 hoare Game1_inv_send_fin: Game1.send_fin:
@@ -639,20 +625,16 @@ hoare Game1_inv_send_fin: Game1.send_fin:
 proof.
 proc; inline *.
 sp; if => //.
-sp; match; 1: auto; 2..4: auto.
+sp; match; 1, 3..5: by auto.
 sp; match.
 - auto => /> &m decn st inv bjin a' i'.
-  case ((a', i') = (b, j){m}) => /> => [|neq_ai].
-  - apply (Game1_aborted _ _ _ _ Responder). smt(get_setE).
-  apply Game1_inv_neq => //.
-  exact inv.
+  exact /Game1_inv_aborted/inv.
 auto => /> &m decn st inv bjin a' i'.
-case ((a', i') = (b, j){m}) => [eq_ai|neq_ai].
+case ((a', i') = (b, j){m}) => [<-|neq_ai].
 + rewrite /get_as_Some //=.
   apply (Game1_accepted _ _ _ _ Responder (m1{m}, m2{m}, m3{m}) (prf (na{m}, nb{m}) (a{m}, b{m}))).
-  - by rewrite get_setE eq_ai //=. 
-apply Game1_inv_neq => //.
-exact inv.
+  by rewrite get_set_sameE. 
+exact /Game1_inv_neq/inv.
 qed.
 
 hoare Game1_inv_rev_skey: Game1.rev_skey:
@@ -662,16 +644,15 @@ hoare Game1_inv_rev_skey: Game1.rev_skey:
 proof.
 proc; inline *.
 sp; if => //.
-sp; match; 1..2: auto; 2..3: auto.
+sp; match; 1,2,4,5: by auto.
 sp; if => //.
 wp 2.
 conseq (: _ ==> true); last by auto.
 move=> /> &m st inv aiin _ k a' i'.
-case ((a', i') = (a, i){m}) => [eq_ai|neq_ai].
+case ((a', i') = (a, i){m}) => [[] <<- <-|neq_ai].
 - apply (Game1_observed _ _ _ _ role{m} trace{m} k).
-smt(get_setE).
-apply Game1_inv_neq => //.
-exact inv.
+  by rewrite get_set_sameE.
+exact /Game1_inv_neq/inv.
 qed.
 
 hoare Game1_inv_test: Game1.test:
@@ -681,16 +662,15 @@ hoare Game1_inv_test: Game1.test:
 proof.
 proc; inline *.
 sp; if => //.
-sp; match; 1..2: auto; 2..3: auto.
+sp; match; 1,2,4,5: by auto.
 sp; if => //.
 wp 2.
 conseq (: _ ==> true); last by auto.
 move=> /> &m st inv aiin _ k a' i'.
-case ((a', i') = (a, i){m}) => [eq_ai|neq_ai].
+case ((a', i') = (a, i){m}) => [[] <<- <-|neq_ai].
 - apply (Game1_observed _ _ _ _ role{m} trace{m} k).
-smt(get_setE).
-apply Game1_inv_neq => //.
-exact inv.
+  by rewrite get_set_sameE.
+exact /Game1_inv_neq/inv.
 qed.
 
 (* ------------------------------------------------------------------------------------------ *)
@@ -704,22 +684,24 @@ proof.
 proc; inline *.
 if => //.
 auto => />.
-move => &m inv1 inv3 k _ a' i'.
-case: (inv1 a' i'). 
-+ move=> sm.
-  by apply Game1_undef.
-+ move => r sm.
-  exact (Game1_aborted _ _ _ _ r).
-+ move => b na c1 kab sm psk.
-  apply (Game1_ipending _ _ _ _ b na c1 kab) => //.
-  smt(get_setE).
-+ move => b na nb c1 c2 kba sm psk.
-  apply (Game1_rpending _ _ _ _ b na nb c1 c2 kba) => //.
-  smt(get_setE).
-+ move => r tr k'.
-  exact (Game1_accepted _ _ _ _ r tr k').
-move => r tr k'.
-exact (Game1_observed _ _ _ _ r tr k').
+move => &m inv abnin pk _ a' i'.
+case: (inv a' i') =>
+[ 
+smbj
+| r smbj
+| b na c1 kab smbj pskcb
+| b na nb c1 c2 kba smbj pskcb
+| r tr k smbj
+| r tr k smbj
+].
++ exact Game1_undef.
++ exact (Game1_aborted _ _ _ _ r).
++ apply (Game1_ipending _ _ _ _ b na c1 kab) => //.
+  by rewrite mem_set pskcb.
++ apply (Game1_rpending _ _ _ _ b na nb c1 c2 kba) => //.
+  by rewrite mem_set pskcb.
++ exact (Game1_accepted _ _ _ _ r tr k).
+exact (Game1_observed _ _ _ _ r tr k).
 qed.
     
 hoare Game2_inv_send_msg1: Game2.send_msg1:
@@ -730,12 +712,10 @@ proof.
 proc; inline *.
 sp; if => //.
 auto => /> &m inv ainin abin ca _ na _ a' i'.
-case ((a', i') = (a, i){m}) => /> => [|neq_ai].
-+ apply (Game1_ipending _ _ _ _ b{m} na ca witness).
-  - by rewrite get_set_sameE.
-  smt().
-apply Game1_inv_neq => //.
-exact inv.
+case ((a', i') = (a, i){m}) => [[] <<- <- |neq_ai].
++ apply (Game1_ipending _ _ _ _ b{m} na ca witness) => //.
+  by rewrite get_set_sameE.
+exact /Game1_inv_neq/inv.
 qed.
     
 hoare Game2_inv_send_msg2: Game2.send_msg2:
@@ -747,18 +727,13 @@ proc; inline *.
 sp; if => //.
 sp; match.
 + auto => /> &m decn st inv bjnin abin a' i'.
-  case ((a', i') = (b, j){m}) => /> => [|neq_ai].
-  - apply (Game1_aborted _ _ _ _ Responder). smt(get_setE).
-  apply Game1_inv_neq => //.
-  exact inv.
+  exact /Game1_inv_aborted/inv.
 auto => /> &m decn st inv bjnin abin cb0 _ n cin a' i'.
-case ((a', i') = (b, j){m}) => [eq_ai|neq_ai].
+case ((a', i') = (b, j){m}) => [[] <<- <-|neq_ai].
 + rewrite /get_as_Some //=.
-  apply (Game1_rpending _ _ _ _ a{m} na{m} n ca{m} cb0 witness).
-  - by rewrite get_setE eq_ai //=. 
-  smt().
-apply Game1_inv_neq => //.
-exact inv.
+  apply (Game1_rpending _ _ _ _ a{m} na{m} n ca{m} cb0 witness) => //.
+  by rewrite get_set_sameE.
+exact /Game1_inv_neq/inv.
 qed.
 
 hoare Game2_inv_send_msg3: Game2.send_msg3:
@@ -771,17 +746,13 @@ sp; if => //.
 sp; match; 2..5: auto.
 sp; match.
 + auto => /> &m decn st inv abin a' i'.
-  case ((a', i') = (a, i){m}) => /> => [|neq_ai].
-  - apply (Game1_aborted _ _ _ _ Initiator). smt(get_setE).
-  apply Game1_inv_neq => //.
-  exact inv.
+  exact /Game1_inv_aborted/inv.
 auto => /> &m decn st inv aiin ca0 _ n cin a' i'.
-case ((a', i') = (a, i){m}) => [eq_ai|neq_ai].
+case ((a', i') = (a, i){m}) => [[] <<- <-|neq_ai].
 + rewrite /get_as_Some //=.
-  apply (Game1_accepted _ _ _ _ Initiator (m1{m}, m2{m}, ca0) (prf (na{m}, nb{m}) (a{m}, b{m}))).
-  - by rewrite get_setE eq_ai //=. 
-apply Game1_inv_neq => //.
-exact inv.
+  apply (Game1_accepted _ _ _ _ Initiator (m1{m}, m2{m}, ca0) (prf (na{m}, nb{m}) (a', b{m}))).
+  by rewrite get_set_sameE. 
+exact /Game1_inv_neq/inv.
 qed.
 
 hoare Game2_inv_send_fin: Game2.send_fin:
@@ -791,20 +762,16 @@ hoare Game2_inv_send_fin: Game2.send_fin:
 proof.
 proc; inline *.
 sp; if => //.
-sp; match; 1: auto; 2..4: auto.
+sp; match; 1, 3..5: by auto.
 sp; match.
 - auto => /> &m decn st inv bjin a' i'.
-  case ((a', i') = (b, j){m}) => /> => [|neq_ai].
-  - apply (Game1_aborted _ _ _ _ Responder). smt(get_setE).
-  apply Game1_inv_neq => //.
-  exact inv.
+  exact /Game1_inv_aborted/inv.
 auto => /> &m decn st inv bjin a' i'.
-case ((a', i') = (b, j){m}) => [eq_ai|neq_ai].
+case ((a', i') = (b, j){m}) => [[] <<- <-|neq_ai].
 + rewrite /get_as_Some //=.
-  apply (Game1_accepted _ _ _ _ Responder (m1{m}, m2{m}, m3{m}) (prf (na{m}, nb{m}) (a{m}, b{m}))).
-  - by rewrite get_setE eq_ai //=. 
-apply Game1_inv_neq => //.
-exact inv.
+  apply (Game1_accepted _ _ _ _ Responder (m1{m}, m2{m}, m3{m}) (prf (na{m}, nb{m}) (a{m}, a'))).
+  by rewrite get_set_sameE.
+exact /Game1_inv_neq/inv.
 qed.
 
 hoare Game2_inv_rev_skey: Game2.rev_skey:
@@ -814,16 +781,15 @@ hoare Game2_inv_rev_skey: Game2.rev_skey:
 proof.
 proc; inline *.
 sp; if => //.
-sp; match; 1..2: auto; 2..3: auto.
+sp; match; 1,2,4,5: by auto.
 sp; if => //.
 wp 2.
 conseq (: _ ==> true); last by auto.
 move=> /> &m st inv aiin _ k a' i'.
-case ((a', i') = (a, i){m}) => [eq_ai|neq_ai].
+case ((a', i') = (a, i){m}) => [[] <<- <-|neq_ai].
 - apply (Game1_observed _ _ _ _ role{m} trace{m} k).
-smt(get_setE).
-apply Game1_inv_neq => //.
-exact inv.
+  by rewrite get_set_sameE.
+exact /Game1_inv_neq/inv.
 qed.
 
 hoare Game2_inv_test: Game2.test:
@@ -833,16 +799,15 @@ hoare Game2_inv_test: Game2.test:
 proof.
 proc; inline *.
 sp; if => //.
-sp; match; 1..2: auto; 2..3: auto.
+sp; match; 1,2,4,5: by auto.
 sp; if => //.
 wp 2.
 conseq (: _ ==> true); last by auto.
 move=> /> &m st inv aiin _ k a' i'.
-case ((a', i') = (a, i){m}) => [eq_ai|neq_ai].
+case ((a', i') = (a, i){m}) => [[] <<- <-|neq_ai].
 - apply (Game1_observed _ _ _ _ role{m} trace{m} k).
-smt(get_setE).
-apply Game1_inv_neq => //.
-exact inv.
+  by rewrite get_set_sameE.
+exact /Game1_inv_neq/inv.
 qed.
 
 (* ------------------------------------------------------------------------------------------ *)
@@ -917,8 +882,17 @@ move=> neq
 + apply (Game3_rpending _ _ _ _ b na nb c1 c2 kba)=> //.
   + smt(get_setE).  
   smt(get_setE).  
-+ exact (Game3_accepted _ _ _ _ r tr k)=> //.
-exact (Game3_observed _ _ _ _ r tr k)=> //.
++ exact (Game3_accepted _ _ _ _ r tr k).
+exact (Game3_observed _ _ _ _ r tr k).
+qed.
+
+lemma Game3_inv_aborted a i b j r sm dm: Game3_inv sm dm a i => Game3_inv sm.[(b, j) <- (r, Aborted)] dm a i.
+proof.
+move=> inv.
+case ((a, i) = (b, j)) => /> => [|neq_ai].
+- apply (Game3_aborted _ _ _ _ r).
+  by rewrite get_set_sameE.
+exact /Game3_inv_neq_sm/inv. 
 qed.
 
 hoare Game3_inv_gen_pskey: Game3.gen_pskey:
@@ -944,12 +918,8 @@ case (Game3.bad).
 sp; if=> //.
 auto => /> &m _ inv ainin abin _ uniq na _ a' i'.
 case ((a', i') = (a, i){m}) => /> => [|neq_ai].
-+ apply (Game3_ipending _ _ _ _ b{m} na ca{m} witness).
-  - by rewrite get_set_sameE.
-  by rewrite get_set_sameE.
-apply Game3_inv_neq_sm => //.
-apply Game3_inv_neq_dm => //.
-exact inv.
++ by apply (Game3_ipending _ _ _ _ b{m} na ca{m} witness); rewrite get_set_sameE.
+exact /Game3_inv_neq_sm/Game3_inv_neq_dm/inv.
 qed.
     
 hoare Game3_inv_send_msg2: Game3.send_msg2:
@@ -961,11 +931,7 @@ proc; inline *.
 sp; if => //.
 sp; match.
 + auto => /> &m decn st inv bjnin abin a' i'.
-  case ((a', i') = (b, j){m}) => /> => [|neq_ai].
-  - apply (Game3_aborted _ _ _ _ Responder).
-    by rewrite get_set_sameE. 
-  apply Game3_inv_neq_sm => //.
-  exact inv.
+  exact /Game3_inv_aborted/inv.
 seq 1 : (#pre); 1: by auto.
 case (Game3.bad).
 + by rcondf ^if; auto=> />.
@@ -974,11 +940,9 @@ auto => /> &m _ decn st inv bjnin abin _ bad n _ a' i'.
 case ((a', i') = (b, j){m}) => /> => [|neq_ai].
 + apply (Game3_rpending _ _ _ _ a{m} na{m} n ca{m} cb{m} witness).
   - by rewrite get_set_sameE.
-  - by rewrite get_set_neqE /#. 
+  - by rewrite get_set_neqE //= decn. 
   by rewrite get_set_sameE.
-apply Game3_inv_neq_sm => //.
-apply Game3_inv_neq_dm => //.
-exact inv.
+exact /Game3_inv_neq_sm/Game3_inv_neq_dm/inv.
 qed.
 
 hoare Game3_inv_send_msg3: Game3.send_msg3:
@@ -991,11 +955,7 @@ sp; if => //.
 sp; match; 2..5: auto.
 sp; match.
 + auto => /> &m decn st inv abin a' i'.
-  case ((a', i') = (a, i){m}) => /> => [|neq_ai].
-  - apply (Game3_aborted _ _ _ _ Initiator).
-    by rewrite get_set_sameE. 
-  apply Game3_inv_neq_sm => //.
-  exact inv.
+  exact /Game3_inv_aborted/inv.
 seq 1 : (#pre); 1: by auto.
 case (Game3.bad).
 + by rcondf ^if; auto=> />.
@@ -1004,9 +964,7 @@ auto => /> &m _ decn st inv aiin _ bad ok _ a' i'.
 case ((a', i') = (a, i){m}) => /> => [|neq_ai].
 + apply (Game3_accepted _ _ _ _ Initiator (m1{m}, m2{m}, caf{m}) (prf (na{m}, nb{m}) (a{m}, b{m}))).
   by rewrite get_set_sameE.
-apply Game3_inv_neq_sm => //.
-apply Game3_inv_neq_dm => //.
-exact inv.
+exact /Game3_inv_neq_sm/Game3_inv_neq_dm/inv.
 qed.
 
 hoare Game3_inv_send_fin: Game3.send_fin:
@@ -1019,17 +977,12 @@ sp; if => //.
 sp; match; 1: auto; 2..4: auto.
 sp; match.
 - auto => /> &m decn st inv bjin a' i'.
-  case ((a', i') = (b, j){m}) => /> => [|neq_ai].
-  - apply (Game3_aborted _ _ _ _ Responder).
-    by rewrite get_set_sameE.
-  apply Game3_inv_neq_sm => //.
-  exact inv.
+  exact /Game3_inv_aborted/inv.
 auto => /> &m decn st inv bjin a' i'.
 case ((a', i') = (b, j){m}) => /> => [|neq_ai].
 + apply (Game3_accepted _ _ _ _ Responder (m1{m}, m2{m}, m3{m}) (prf (na{m}, nb{m}) (a{m}, b{m}))).
   by rewrite get_set_sameE. 
-apply Game3_inv_neq_sm => //.
-exact inv.
+exact /Game3_inv_neq_sm/inv.
 qed.
 
 hoare Game3_inv_rev_skey: Game3.rev_skey:
@@ -1039,7 +992,7 @@ hoare Game3_inv_rev_skey: Game3.rev_skey:
 proof.
 proc; inline *.
 sp; if => //.
-sp; match; 1..2: auto; 2..3: auto.
+sp; match; 1,2,4,5: by auto.
 sp; if => //.
 wp 2.
 conseq (: _ ==> true); last by auto.
@@ -1047,8 +1000,7 @@ move=> /> &m st inv aiin _ k a' i'.
 case ((a', i') = (a, i){m}) => /> => [|neq_ai].
 - apply (Game3_observed _ _ _ _ role{m} trace{m} k).
   by rewrite get_set_sameE. 
-apply Game3_inv_neq_sm => //.
-exact inv.
+exact /Game3_inv_neq_sm/inv.
 qed.
 
 hoare Game3_inv_test: Game3.test:
@@ -1058,7 +1010,7 @@ hoare Game3_inv_test: Game3.test:
 proof.
 proc; inline *.
 sp; if => //.
-sp; match; 1..2: auto; 2..3: auto.
+sp; match; 1,2,4,5: by auto.
 sp; if => //.
 wp 2.
 conseq (: _ ==> true); last by auto.
@@ -1066,6 +1018,274 @@ move=> /> &m st inv aiin _ k a' i'.
 case ((a', i') = (a, i){m}) => /> => [|neq_ai].
 - apply (Game3_observed _ _ _ _ role{m} trace{m} k).
   by rewrite get_set_sameE. 
-apply Game3_inv_neq_sm => //.
-exact inv.
+exact /Game3_inv_neq_sm/inv.
+qed.
+
+(* ------------------------------------------------------------------------------------------ *)
+(* Game 5 invariants *)
+inductive Game5_inv 
+  (sm: (id * int, role * instance_state) fmap)
+  (dm : ((id * id) * msg_data * ctxt, nonce) fmap)
+  (nm : (msg_data * ctxt, nonce * nonce) fmap)
+  (a: id) (i: int)
+=
+| Game5_undef of
+    (sm.[a, i] = None)
+| Game5_aborted r of
+    (sm.[a, i] = Some (r, Aborted))
+| Game5_ipending b c1 of
+    (sm.[a, i] = Some (Initiator, IPending (b, witness, witness, c1) (a, c1)))
+  & (((a, b), msg1_data a b, c1) \in dm)
+  & (forall c2 c3, (msg3_data a b c1 c2, c3) \notin nm)
+| Game5_rpending b c1 c2 of
+    (sm.[a, i] = Some (Responder, RPending (b, witness, witness, witness, c1, c2) (b, c1) c2))
+| Game5_accepted r tr k of
+    (sm.[a, i] = Some (r, Accepted tr k))
+| Game5_observed r tr k of
+    (sm.[a, i] = Some (r, Observed tr k)).
+   
+op Game5_inv_full
+  (sm: (id * int, role * instance_state) fmap)
+  (dm : ((id * id) * msg_data * ctxt, nonce) fmap)
+  (nm : (msg_data * ctxt, nonce * nonce) fmap)
+=
+  ((forall a i j b c, 
+       sm.[(a, i)] = Some (Initiator, IPending (b, witness, witness, c) (a, c))
+    /\ sm.[(a, j)] = Some (Initiator, IPending (b, witness, witness, c) (a, c))
+    => i = j)
+  /\ (forall a b ca cb, ((a, b), msg2_data a b ca, cb) \in dm => ((a, b), msg1_data a b, ca) \in dm)
+  /\ (forall a b ca cb caf, ((a, b), msg3_data a b ca cb, caf) \in dm => ((a, b), msg2_data a b ca, cb) \in dm)
+  /\ (forall a b ca cb caf, (msg3_data a b ca cb, caf) \in nm <=> ((a, b), msg3_data a b ca cb, caf) \in dm))
+  /\ (forall a i, Game5_inv sm dm nm a i).
+
+lemma Game5_inv_neq_sm a i c j v sm dm nm:
+! (c = a /\ j = i) =>
+Game5_inv sm dm nm c j =>
+Game5_inv sm.[(a, i) <- v] dm nm c j.
+proof.
+move=> neq
+[ 
+  smbj
+| r smbj
+| b c1 smbj
+| b c1 c2 smbj
+| r tr k smbj
+| r tr k smbj
+].
++ apply Game5_undef.
+  by rewrite get_set_neqE.
++ apply (Game5_aborted _ _ _ _ _ r).
+  by rewrite get_set_neqE.
++ apply (Game5_ipending _ _ _ _ _ b c1) => //.
+  by rewrite get_set_neqE.
++ apply (Game5_rpending _ _ _ _ _ b c1 c2)=> //.
+  by rewrite get_set_neqE.
++ apply (Game5_accepted _ _ _ _  _ r tr k)=> //.
+  by rewrite get_set_neqE.
+apply (Game5_observed _ _ _ _ _ r tr k)=> //.
+by rewrite get_set_neqE.
+qed.
+
+lemma Game5_inv_neq_dm a i m sm (dm : (_, _) fmap) nm:
+! (exists pk ad, (pk, ad, m) \in dm) =>
+Game5_inv sm dm nm a i =>
+forall pk ad, Game5_inv sm dm.[(pk, ad, m) <- witness] nm a i.
+proof.
+move=> neq
+[ 
+  smbj
+| r smbj
+| b c1 smbj v1 v2
+| b c1 c2 smbj
+| r tr k smbj
+| r tr k smbj
+] pk ad.
++ exact Game5_undef.
++ exact (Game5_aborted _ _ _ _ _ r).
++ apply (Game5_ipending _ _ _ _ _ b c1) => //.
+  by rewrite mem_set v1.  
++ exact (Game5_rpending _ _ _ _ _ b c1 c2).
++ exact (Game5_accepted _ _ _ _  _ r tr k).
+exact (Game5_observed _ _ _ _ _ r tr k).
+qed.
+
+lemma Game5_inv_aborted a i b j r sm dm nm: Game5_inv sm dm nm a i => Game5_inv sm.[(b, j) <- (r, Aborted)] dm nm a i.
+proof.
+move=> inv.
+case ((a, i) = (b, j)) => /> => [|neq_ai].
+- apply (Game5_aborted _ _ _ _ _ r).
+  by rewrite get_set_sameE.
+exact /Game5_inv_neq_sm/inv. 
+qed.
+
+hoare Game5_inv_send_msg1: Game5.send_msg1:
+  (Game5_inv_full Game5.state_map Game5.dec_map Game5.prfkey_map)
+  ==>
+  (Game5_inv_full Game5.state_map Game5.dec_map Game5.prfkey_map).
+proof.
+proc.
+sp; if=> //.
+seq 1 : (#pre); 1: by auto.
+case (Game5.bad).
++ by rcondf ^if; auto=> />.
+auto=> />.
+move=> &m inv1 inv2 inv3 inv4 inv5 ainin abin _ canin.
+split.
++ split; 2: smt(get_setE).
+  move=> a' i' j b' c.
+  rewrite !get_setE //=.
+  case: (a' = a{m}) => />; last by smt().
+  case: (i' = i{m}) => />.
+  + case: (j = i{m}) => />.
+    move=> neqji smj.
+    case: (inv5 a{m} j); rewrite smj //=.
+    smt().
+  move=> neqi'i smi.
+  case: (inv5 a{m} i'); rewrite smi //=.
+  smt().
+move=> a i.
+case: ((a, i) = (a, i){!m}) => /> => [| neq].
++ apply (Game5_ipending _ _ _ _ _ b{m} ca{m}).
+  + by rewrite get_set_sameE.
+  + by rewrite mem_set.
+  smt().
+exact /Game5_inv_neq_sm/Game5_inv_neq_dm/inv5.
+qed.
+
+hoare Game5_inv_send_msg2: Game5.send_msg2:
+  (Game5_inv_full Game5.state_map Game5.dec_map Game5.prfkey_map)
+  ==>
+  (Game5_inv_full Game5.state_map Game5.dec_map Game5.prfkey_map).
+proof.
+proc.
+sp; if=> //.
+sp; match => //.
++ auto=> />.
+  move=> &m dm sm inv1 inv2 inv3 inv4 inv5 bjnin abin.
+  split; 1: smt(get_setE).
+  move=> b j.
+  exact /Game5_inv_aborted/inv5.
+seq 1 : (#pre); 1: by auto.
+case (Game5.bad).
++ by rcondf ^if; auto=> />.
+auto=> />.
+move=> &m dm sm inv1 inv2 inv3 inv4 inv5 bjnin abin _ cbnin.
+split; 1: smt(get_setE).
+move=> b j.
+case: ((b, j) = (b, j){!m}) => /> => [|neq_ai].
+- apply (Game5_rpending _ _ _ _ _ a{m} ca{m} cb{m}).
+  by rewrite get_set_sameE. 
+exact /Game5_inv_neq_sm/Game5_inv_neq_dm/inv5.
+qed.
+
+hoare Game5_inv_send_msg3: Game5.send_msg3:
+  (Game5_inv_full Game5.state_map Game5.dec_map Game5.prfkey_map)
+  ==>
+  (Game5_inv_full Game5.state_map Game5.dec_map Game5.prfkey_map).
+proof.
+proc.
+sp; if=> //.
+sp; match => //.
+sp; match => //.
++ auto=> />.
+  move=> &m dm sm inv1 inv2 inv3 inv4 inv5 aiin.
+  split; 1: smt(get_setE).
+  move=> a i.
+  exact /Game5_inv_aborted/inv5.
+seq 1 : (#pre); 1: by auto.
+case (Game5.bad).
++ by rcondf ^if; auto=> />.
+sp; if=> //.
+auto=> />.
+move=> &m _ dm sm inv1 inv2 inv3 inv4 inv5 /domE aiin _ cafnin ns _.
+split; 1: smt(get_setE).
+move=> a' i'.
+case: ((a', i') = (a, i){m}) => /> => [|neq_ai].
+- apply (Game5_accepted _ _ _ _ _ Initiator (m1, m2, caf){m} (prf (ns.`1, ns.`2) (a, b)){!m}).
+  by rewrite get_set_sameE. 
+apply /Game5_inv_neq_sm/Game5_inv_neq_dm => //=.
+case: (inv5 a' i') =>
+[ 
+  smai
+| r smai
+| b c1 smai' v1 v2
+| b c1 c2 smai
+| r tr k smai
+| r tr k smai
+].
++ exact Game5_undef.
++ exact (Game5_aborted _ _ _ _ _ r).
++ apply (Game5_ipending _ _ _ _ _ b c1) => //.
+  move=> c2 c3.
+  have smai : Game5.state_map{m}.[(a, i){m}] = Some (role{m}, IPending (b{!m}, psk{m}, na{m}, ca{m}) m1{m}).
+  + by rewrite some_oget //= -sm.
+  case: (inv5 a{m} i{m}); rewrite smai //=.
+  smt(mem_set).
++ exact (Game5_rpending _ _ _ _ _ b c1 c2).
++ exact (Game5_accepted _ _ _ _  _ r tr k).
+exact (Game5_observed _ _ _ _ _ r tr k).
+qed.
+
+hoare Game5_inv_send_fin: Game5.send_fin:
+  (Game5_inv_full Game5.state_map Game5.dec_map Game5.prfkey_map)
+  ==>
+  (Game5_inv_full Game5.state_map Game5.dec_map Game5.prfkey_map).
+proof.
+proc.
+sp; if=> //.
+sp; match => //.
+sp; match => //.
++ auto=> />.
+  move=> &m dm sm inv1 inv2 inv3 inv4 inv5 bjin.
+  split; 1: smt(get_setE).
+  move=> b j.
+  exact /Game5_inv_aborted/inv5.
+auto=> />.
+move=> &m dm sm inv1 inv2 inv3 inv4 inv5 /domE bjin.
+split; 1: smt(get_setE).
+move=> b' j'.
+case ((b', j') = (b, j){m}) => /> => [|neq_bj].
+- apply (Game5_accepted _ _ _ _ _ Responder (m1, m2, m3){m} (prf (oget Game5.prfkey_map{m}.[(msg3_data a{m} b{m} ca{m} cb{m}, m3{m})]) (a, b)){m}).
+  by rewrite get_set_sameE. 
+exact /Game5_inv_neq_sm/inv5. 
+qed.
+
+hoare Game5_inv_rev_skey: Game5.rev_skey:
+  (Game5_inv_full Game5.state_map Game5.dec_map Game5.prfkey_map)
+  ==>
+  (Game5_inv_full Game5.state_map Game5.dec_map Game5.prfkey_map).
+proof.
+proc.
+sp; if=> //.
+sp; match => //; 2: by auto.
+sp; if=> //.
+wp 2.
+conseq (: _ ==> true); last by auto.
+auto => /> &m st inv1 inv2 inv3 inv4 inv5 aiin _ k.
+split; 1: smt(get_setE).
+move=> a' i'.
+case ((a', i') = (a, i){m}) => /> => [|neq_ai].
+- apply (Game5_observed _ _ _ _ _ role{m} trace{m} k).
+  by rewrite get_set_sameE.
+exact /Game5_inv_neq_sm/inv5. 
+qed.
+
+hoare Game5_inv_test: Game5.test:
+  (Game5_inv_full Game5.state_map Game5.dec_map Game5.prfkey_map)
+  ==>
+  (Game5_inv_full Game5.state_map Game5.dec_map Game5.prfkey_map).
+proof.
+proc.
+sp; if=> //.
+sp; match => //; 2: by auto.
+sp; if=> //.
+wp 2.
+conseq (: _ ==> true); last by auto.
+auto => /> &m st inv1 inv2 inv3 inv4 inv5 aiin _ k.
+split; 1: smt(get_setE).
+move=> a' i'.
+case ((a', i') = (a, i){m}) => /> => [|neq_ai].
+- apply (Game5_observed _ _ _ _ _ role{m} trace{m} k).
+  by rewrite get_set_sameE.
+exact /Game5_inv_neq_sm/inv5. 
 qed.
