nsl/Security.ec
@@ -5,8 +5,26 @@ import GWAKEc AEADc PRFc.
 (* Reductions *)
 (* ------------------------------------------------------------------------------------------ *)
 
+print Game1.
 (* AEAD Reduction *)
 module (Red_AEAD (D : A_GWAKE) : A_GAEAD) (O : GAEAD_out) = {
+  (*
+  module WAKE_O : GWAKE_out = Game1 with {
+    var - psk_map
+    
+    proc init_mem [ ^psk_map<- - ]
+    proc gen_pskey ~ O.gen
+    proc send_msg1
+    (ex : bool)
+    [
+      ^mo<- + { ex <@ O.ex((a, b)); },
+      ^if ~ ((a, i) \notin state_map /\ ex),
+      ^if.^ca<$ -,
+      ^if.^mo<- ~ { mo <@ O.enc((a, b), msg1_data a b, na); ca <- oget mo; }
+    ]
+    
+  }
+  *)
   module WAKE_O : GWAKE_out = {
     var state_map: (id * int, role * instance_state) fmap
   
@@ -26,9 +44,8 @@ module (Red_AEAD (D : A_GWAKE) : A_GAEAD) (O : GAEAD_out) = {
         mo <@ O.enc((a, b), msg1_data a b, na);
         state_map.[(a, i)] <- (Initiator, IPending (b, witness, na, oget mo) (a, oget mo));
       }
-      return (mo);
+      return mo;
     }
-
 
     proc send_msg2(b, j, m1) = {
       var a, ca, role, st, ex, n, nb;
@@ -102,13 +119,10 @@ module (Red_AEAD (D : A_GWAKE) : A_GAEAD) (O : GAEAD_out) = {
         match st with
         | Accepted trace k' => {
           k <- k';
-          (* Get partners *)
           ps <- get_partners (a, i) (Some trace) role state_map;
           if (card ps <= 1) {
             ps <- get_observed_partners (a, i) state_map;
-            (* If we have no observed partners then, we can test *)
             if (card ps <> 0) {
-              (* If a partner has revealed something, we must use the same key *)
               p <- pick ps;
               (p_role, p_st) <- oget state_map.[p];
               if (p_st is Observed _ p_k) {
@@ -151,173 +165,36 @@ clone import PROM.FullRO as NROc with
 proof *.
 
 module (Red_ROM (D : A_GWAKE) : RO_Distinguisher) (O : RO) = {
-  module WAKE_O : GWAKE_out = {
-    var dec_map : ((id * id) * msg_data * ctxt, nonce) fmap
-    var bad : bool
-    var state_map : (id * int, role * instance_state) fmap
-    var psk_map : (id * id, pskey) fmap
-  
-    proc init_mem() = {
-      state_map <- empty;
-      psk_map <- empty;
-      bad <- false;
-      dec_map <- empty;
-    }
-  
-    proc gen_pskey(a, b) = {
-      var k;
-  
-      if ((a, b) \notin psk_map) {
-        k <$ dpskey;
-        psk_map.[a, b] <- k;
+  module WAKE_O : GWAKE_out = Game4 with {
+    proc send_msg1 [
+      ^if.^if.^na<$ ~ {na <- witness; O.sample((msg1_data a b, ca)); }
+    ]
+
+    proc send_msg2 [
+      ^if.^match#Some.^if.^nb<$ ~ {nb <- witness; O.sample((msg2_data a b ca, cb)); }
+    ]
+
+    proc send_msg3 [
+      ^if.^match#IPending.^match#Some.^if.^ok<$ ~ {
+        ok <- witness;
+        O.sample((msg3_data a b ca m2, caf));
+      },
+      ^if.^match#IPending.^match#Some.^if.^skey<- ~ {
+        na <@ O.get((msg1_data a b, ca));
+        ok <@ O.get((msg2_data a b ca, m2));
+        skey <- prf (na, ok) (a, b);
       }
-    }
-  
-    proc send_msg1(a, i, b) = {
-      var ca, mo;
-      
-      mo <- None;
-      if (((a, i) \notin state_map) /\ ((a, b) \in psk_map)) {
-        ca <$ dctxt;
-        bad <- bad \/ exists pk ad, (pk, ad, ca) \in dec_map;
-        if (!bad) {
-          O.sample((msg1_data a b, ca));
-          dec_map.[(a, b), msg1_data a b, ca] <- witness;
-          mo <- Some ca;
-          state_map.[a, i] <- (Initiator, IPending (b, witness, witness, ca) (a, ca));
-        }
+    ]
+
+    proc send_fin [
+      ^if.^match#RPending.^match#Some.^skey<- ~ {
+        na <@ O.get((msg1_data a b, ca));
+        nb <@ O.get((msg2_data a b ca, cb));
+        skey <- prf (na, nb) (a, b);
       }
-      
-      return mo;
-    }
-    
-    proc send_msg2(b : id, j : int, m1 : id * ctxt) : ctxt option = {
-      var a, ca, role, st, cb, mo;
-      
-      mo <- None;
-      (a, ca) <- m1;
-      (role, st) <- oget state_map.[b, j];
-      if (((b, j) \notin state_map) /\ ((a, b) \in psk_map)) {
-        if (dec_map.[(a, b), msg1_data a b, ca] is Some na) {
-          cb <$ dctxt;
-          bad <- bad \/ exists pk ad, (pk, ad, cb) \in dec_map;
-          if (!bad) {
-            O.sample((msg2_data a b ca, cb));
-            dec_map.[(a, b), msg2_data a b ca, cb] <- witness;
-            mo <- Some cb;
-            state_map.[b, j] <- (Responder, RPending (a, witness, witness, witness, ca, cb) m1 cb);
-          }
-        } else {
-          state_map.[b, j] <- (Responder, Aborted);
-        }
-      }
-      
-      return mo;
-    }
-    
-    proc send_msg3(a : id, i : int, m2 : ctxt) : ctxt option = {
-      var role, st, b, psk, na, ok, ca, skey, caf, mo; 
-      
-      mo <- None;
-      if ((a, i) \in state_map) {
-        (role, st) <- oget state_map.[a, i];
-        match (st) with
-        | IPending s m1 => {
-          (b, psk, na, ca) <- s;
-          if (dec_map.[(a, b), msg2_data a b ca, m2] is Some nb) {
-            caf <$ dctxt;
-            bad <- bad \/ exists pk ad, (pk, ad, caf) \in dec_map;
-            if (!bad) {
-              O.sample((msg3_data a b ca m2, caf));
-              dec_map.[(a, b), msg3_data a b ca m2, caf] <- witness;
-              mo <- Some caf;
-              na <@ O.get((msg1_data a b, ca));
-              ok <@ O.get((msg2_data a b ca, m2));
-              skey <- prf (na, ok) (a, b);
-              state_map.[a, i] <- (Initiator, Accepted (m1, m2, caf) skey);
-            }
-          } else {
-            state_map.[a, i] <- (Initiator, Aborted);
-          }
-        }
-        | RPending _ _ _ => {}
-        | Accepted _ _ => {}
-        | Observed _ _ => {}
-        | Aborted => {}
-        end;
-      }
-      
-      return mo;
-    }
-    
-    proc send_fin(b : id, j : int, m3 : ctxt) : unit option = {
-      var role, st, a, psk, na, nb, ca, cb, skey, mo;
-      
-      mo <- None;
-      if ((b, j) \in state_map) {
-        (role, st) <- oget state_map.[b, j];
-        match (st) with
-        | IPending _ _ => {}
-        | RPending s m1 m2 => {
-          (a, psk, na, nb, ca, cb) <- s;
-          if(dec_map.[(a, b), msg3_data a b ca cb, m3] is Some nok) {
-            na <@ O.get((msg1_data a b, ca));
-            nb <@ O.get((msg2_data a b ca, cb));
-            skey <- prf (na, nb) (a, b);
-            state_map.[b, j] <- (Responder, Accepted (m1, m2, m3) skey);
-            mo <- Some tt;
-          } else {
-           state_map.[b, j] <- (Responder, Aborted);
-          }
-        }
-        | Accepted _ _ => {}
-        | Observed _ _ => {}
-        | Aborted => {}
-        end;
-      }
-      
-      return mo;
-    }
-  
-    proc rev_skey(a, i) = {
-      var role, st, p_role, p_st, ps, p, k;
-      var ko <- None;
-    
-      if ((a, i) \in state_map) {
-        (role, st) <- oget state_map.[(a, i)];
-        match st with
-        | Accepted trace k' => {
-          k <- k';
-          (* Get partners *)
-          ps <- get_partners (a, i) (Some trace) role state_map;
-          if (card ps <= 1) {
-            ps <- get_observed_partners (a, i) state_map;
-            (* If we have no observed partners then, we can test *)
-            if (card ps <> 0) {
-              (* If a partner has revealed something, we must use the same key *)
-              p <- pick ps;
-              (p_role, p_st) <- oget state_map.[p];
-              if (p_st is Observed _ p_k) {
-                k <- p_k;
-              }
-            }
-            ko <- Some k;
-            state_map.[(a, i)] <- (role, Observed trace k);
-          }
-        }
-        | Observed _ k'  => ko <- Some k';
-        | IPending _ _   => { }
-        | RPending _ _ _ => { }
-        | Aborted        => { }
-        end;
-      }
-      return ko;
-    }
-    
-    proc test = rev_skey
+    ]
   }
 
-  
   proc distinguish() = {
     var b;
     WAKE_O.init_mem();
@@ -623,564 +500,505 @@ auto => />.
 qed.
 
 (* ------------------------------------------------------------------------------------------ *)
-(* Red_ROM invariants *)
-inductive Red_ROM_inv 
-  (sm: (id * int, role * instance_state) fmap)
-  (dm : ((id * id) * msg_data * ctxt, nonce) fmap)
-  (nm : (msg_data * ctxt, nonce) fmap)
-  (a: id) (i: int)
-=
-| Red_ROM_undef of
-    (sm.[a, i] = None)
-| Red_ROM_aborted r of
-    (sm.[a, i] = Some (r, Aborted))
-| Red_ROM_ipending b c1 of
-    (sm.[a, i] = Some (Initiator, IPending (b, witness, witness, c1) (a, c1)))
-  & (((a, b), msg1_data a b, c1) \in dm)
-  & ((msg1_data a b, c1) \notin nm)
-  & (forall c2, (msg2_data a b c1, c2) \notin nm)
-| Red_ROM_rpending b c1 c2 of
-    (sm.[a, i] = Some (Responder, RPending (b, witness, witness, witness, c1, c2) (b, c1) c2))
-  & (forall c3, ((b, a), msg3_data b a c1 c2, c3) \in dm => (msg1_data b a, c1) \in nm /\ (msg2_data b a c1, c2) \in nm)
-| Red_ROM_accepted r tr k of
-    (sm.[a, i] = Some (r, Accepted tr k))
-| Red_ROM_observed r tr k of
-    (sm.[a, i] = Some (r, Observed tr k)).
-   
-lemma Red_ROM_inv_neq_sm a i c j v sm dm nm:
-! (c = a /\ j = i) =>
-Red_ROM_inv sm dm nm c j =>
-Red_ROM_inv sm.[(a, i) <- v] dm nm c j.
+(* Step 0: Inline procedure calls, and remove pskeys from the state using psk_map to retrieve. *)
+
+local op clear_psk (s : instance_state) =
+match s with
+| IPending st m1 => 
+  let (id, psk, na, ca) = st in IPending (id, witness, na, ca) m1 
+| RPending st m1 m2 => 
+  let (id, psk, na, nb, ca, cb) = st in RPending (id, witness, na, nb, ca, cb) m1 m2 
+| Accepted _ _ => s
+| Observed _ _ => s
+| Aborted => s
+end.
+
+local lemma eq_partners h tr r sml smr: 
+  (forall h, omap (fun (v: role * instance_state) => let (r, s) = v in (r, clear_psk s)) sml.[h] = smr.[h]) =>
+get_partners h tr r sml = get_partners h tr r smr.
 proof.
-move=> neq
-[ 
-  smbj
-| r smbj
-| b c1 smbj
-| b c1 c2 smbj
-| r tr k smbj
-| r tr k smbj
-].
-+ apply Red_ROM_undef.
-  by rewrite get_set_neqE.
-+ apply (Red_ROM_aborted _ _ _ _ _ r).
-  by rewrite get_set_neqE.
-+ apply (Red_ROM_ipending _ _ _ _ _ b c1) => //.
-  by rewrite get_set_neqE.
-+ apply (Red_ROM_rpending _ _ _ _ _ b c1 c2)=> //.
-  by rewrite get_set_neqE.
-+ apply (Red_ROM_accepted _ _ _ _  _ r tr k)=> //.
-  by rewrite get_set_neqE.
-apply (Red_ROM_observed _ _ _ _ _ r tr k)=> //.
-by rewrite get_set_neqE.
+move=> eqsm.
+rewrite /get_partners.
+congr.
+apply fmap_eqP => h'.
+rewrite !filterE -(eqsm h') /=. 
+case: (sml.[h'])=> //=.
+by move=> [r' []] // [] /= /#.
 qed.
 
-op Red_ROM_full_inv sm dm nm : bool =
-  (forall a i, Red_ROM_inv sm dm nm a i)
-  /\ (forall a i j b psk na c, 
-       sm.[(a, i)] = Some (Initiator, IPending (b, psk, na, c) (a, c))
-    /\ sm.[(a, j)] = Some (Initiator, IPending (b, psk, na, c) (a, c))
-    => i = j)
-  /\ (forall a b ca cb, (msg2_data a b ca, cb) \in nm => (msg1_data a b, ca) \in nm)
-  /\ (forall a b ca, (msg1_data a b, ca) \in nm => ((a, b), msg1_data a b, ca) \in dm)
-  /\ (forall a b ca cb, (msg2_data a b ca, cb) \in nm => ((a, b), msg2_data a b ca, cb) \in dm)
-  /\ (forall a b ca cb, ((a, b), msg2_data a b ca, cb) \in dm => ((a, b), msg1_data a b, ca) \in dm)
-  /\ (forall a b ca cb caf, ((a, b), msg3_data a b ca cb, caf) \in dm => (msg2_data a b ca, cb) \in nm)
-.
-
-hoare Red_ROM_inv_send_msg1: Red_ROM(A, LRO).WAKE_O.send_msg1:
-  Red_ROM_full_inv Red_ROM.WAKE_O.state_map Red_ROM.WAKE_O.dec_map RO.m
-==>
-  Red_ROM_full_inv Red_ROM.WAKE_O.state_map Red_ROM.WAKE_O.dec_map RO.m.
+local lemma eq_obs_partners h sml smr: 
+  (forall h, omap (fun (v: role * instance_state) => let (r, s) = v in (r, clear_psk s)) sml.[h] = smr.[h]) =>
+get_observed_partners h sml = get_observed_partners h smr.
 proof.
+move=> eqsm.
+rewrite /get_observed_partners.
+congr.
++ rewrite fun_ext => bj.
+  rewrite -(eqsm bj) //=.
+  case: (sml.[bj])=> //.
+  by move=> [r' []] // [].
+rewrite -(eq_partners _ _ _ sml smr eqsm). 
+rewrite -(eqsm h) /s /r //=.
+case: (sml.[h])=> //.
+by move=> [r' []] // [].
+qed.
+
+lemma Step0 &m:
+    Pr[E_GWAKE(GWAKE0(NSL), A).run() @ &m : res] = Pr[E_GWAKE(Game1, A).run() @ &m : res].
+proof.
+byequiv => //.
 proc; inline*.
-sp; if=> //.
-seq 1 : (#pre); 1: by auto.
-case (Red_ROM.WAKE_O.bad).
-+ by rcondf ^if; auto=> />.
+call (:
+    ={psk_map}(GWAKEb, Game1)
+/\ (forall h, omap (fun v => let (r, s) = v in (r, clear_psk s)) GWAKEb.state_map.[h]{1} = Game1.state_map.[h]{2})
+/\ (forall a i, GWAKE0_inv GWAKEb.state_map GWAKEb.psk_map a i){1}
+).
+- conseq (: ={res}
+          /\ ={psk_map}(GWAKEb, Game1)
+          /\ (forall h, omap (fun v => let (r, s) = v in (r, clear_psk s)) GWAKEb.state_map.[h]{1} = Game1.state_map.[h]{2})
+  ) GWAKE0_inv_gen_pskey _ => //.
+  proc.
+  by if; auto.
+
+- conseq (: ={res}
+          /\ ={psk_map}(GWAKEb, Game1)
+          /\ (forall h, omap (fun v => let (r, s) = v in (r, clear_psk s)) GWAKEb.state_map.[h]{1} = Game1.state_map.[h]{2})
+  ) GWAKE0_inv_send_msg1 _ => //.
+  proc; inline.
+  sp; if=> //.
+  + smt().
+  auto=> />.
+  smt(get_setE).
+
+- conseq (: ={res}
+          /\ ={psk_map}(GWAKEb, Game1)
+          /\ (forall h, omap (fun v => let (r, s) = v in (r, clear_psk s)) GWAKEb.state_map.[h]{1} = Game1.state_map.[h]{2})
+  ) GWAKE0_inv_send_msg2 _ => //.
+  proc; inline.
+  sp; if=> //.
+  + smt().
+  sp; match =.
+  + smt().
+  + auto=> />.
+    smt(get_setE).
+  move=> na.
+  by match Some {1} ^match; auto; smt(get_setE).
+
+- conseq (: ={res}
+          /\ ={psk_map}(GWAKEb, Game1)
+          /\ (forall h, omap (fun v => let (r, s) = v in (r, clear_psk s)) GWAKEb.state_map.[h]{1} = Game1.state_map.[h]{2})
+  ) GWAKE0_inv_send_msg3 _ => //.
+  proc; inline.
+  sp; if=> //.
+  + smt().
+  sp; match; 1..5: smt(); 2..5: by auto.
+  move=> sil m1l sir m1r.
+  sp; match =.
+  + auto=> />.
+    move=> &1 &2 smr sml inv_sm invl ai_in.
+    case: (invl a{2} i{2})=> /#.
+  + match None {1} ^match; auto; smt(get_setE).
+  move=> nb.
+  match Some {1} ^match.
+  + auto; smt(get_setE).
+  auto=> />.
+  move=> &1 &2 + + + sml + invl.
+  case: (invl a{2} i{2}); 1,2,4,5,6: smt().
+  smt(get_setE).
+
+- conseq (: ={res}
+          /\ ={psk_map}(GWAKEb, Game1)
+          /\ (forall h, omap (fun v => let (r, s) = v in (r, clear_psk s)) GWAKEb.state_map.[h]{1} = Game1.state_map.[h]{2})
+  ) GWAKE0_inv_send_fin _ => //.
+  proc; inline.
+  sp; if=> //.
+  + smt().
+  sp; match; 1..5: smt(); 1,3,4,5: by auto.
+  move=> sil m1l m2l sir m1r m2r.
+  sp; match =.
+  + auto=> />. 
+    move=> &1 &2 smr sml inv_sm invl bj_in.
+    case: (invl b{2} j{2})=> /#.
+  + match None {1} ^match; auto; smt(get_setE).
+  move=> nb.
+  match Some {1} ^match.
+  + auto; smt(get_setE).
+  auto=> />.
+  move=> &1 &2 + + + sml + invl.
+  case: (invl b{2} j{2}); 1,2,3,5,6: smt().
+  smt(get_setE).
+
+- conseq (: ={res}
+          /\ ={psk_map}(GWAKEb, Game1)
+          /\ (forall h, omap (fun v => let (r, s) = v in (r, clear_psk s)) GWAKEb.state_map.[h]{1} = Game1.state_map.[h]{2})
+  ) GWAKE0_inv_rev_skey _ => //.
+  proc; inline. 
+  sp; if=> //.
+  + smt().
+  sp; match; 1..5: smt(); 1,2,5: by auto.
+  + move=> tr k tr' k'.
+    sp ^if & -1 ^if & -1; if=> //.
+    + smt(eq_partners).
+    sp ^if & -1 ^if & -1; if.
+    + move=> /> &1 &2 smr sml eqsm.
+      by rewrite (eq_obs_partners (a, i){2} GWAKEb.state_map{1} Game1.state_map{2}).
+    + seq 1 1 : (={ps, p} /\ #pre).
+      + auto=> /> &1 &2 smr sml eqsm.
+        by rewrite (eq_obs_partners (a, i){2} GWAKEb.state_map{1} Game1.state_map{2}).
+      wp 2 2.
+      conseq (: _ ==> ={k, role} /\ tr = tr').
+      + move=> /> &1 &2 _ + + eqsm invl a_in _ _.
+        rewrite -(eqsm (a, i){2}).
+        by case: (GWAKEb.state_map{1}.[(a, i){2}]); smt(get_setE).
+      auto=> /> &1 &2 + + + eqsm invl a_in _ _.
+      rewrite -(eqsm (a, i){2}) -(eqsm p{2}).
+      case: (GWAKEb.state_map{1}.[(a, i){2}])=> />.
+      + by case: (GWAKEb.state_map{1}.[p{2}])=> /#.
+      by case: (GWAKEb.state_map{1}.[p{2}])=> /#.
+    auto=> /> &1 &2 + + eqsm invl a_in _ _.
+    rewrite -(eqsm (a, i){2}).
+    by case: (GWAKEb.state_map{1}.[(a, i){2}]); smt(get_setE).
+  by auto; smt().
+
+- conseq (: ={res}
+          /\ ={psk_map}(GWAKEb, Game1)
+          /\ (forall h, omap (fun v => let (r, s) = v in (r, clear_psk s)) GWAKEb.state_map.[h]{1} = Game1.state_map.[h]{2})
+     ) GWAKE0_inv_test _ => //.
+  proc; inline. 
+  sp; if=> //.
+  + smt().
+  sp; match; 1..5: smt(); 1,2,5: by auto.
+  + move=> tr k tr' k'.
+    sp ^if & -1 ^if & -1; if=> //.
+    + smt(eq_partners).
+    sp ^if & -1 ^if & -1; if.
+    + move=> /> &1 &2 smr sml eqsm.
+      by rewrite (eq_obs_partners (a, i){2} GWAKEb.state_map{1} Game1.state_map{2}).
+    + seq 1 1 : (={ps, p} /\ #pre).
+      + auto=> /> &1 &2 smr sml eqsm.
+        by rewrite (eq_obs_partners (a, i){2} GWAKEb.state_map{1} Game1.state_map{2}).
+      wp 2 2.
+      conseq (: _ ==> ={k, role} /\ tr = tr').
+      + move=> /> &1 &2 _ + + eqsm invl a_in _ _.
+        rewrite -(eqsm (a, i){2}).
+        by case: (GWAKEb.state_map{1}.[(a, i){2}]); smt(get_setE).
+      auto=> /> &1 &2 + + + eqsm invl a_in _ _.
+      rewrite -(eqsm (a, i){2}) -(eqsm p{2}).
+      case: (GWAKEb.state_map{1}.[(a, i){2}])=> />.
+      + by case: (GWAKEb.state_map{1}.[p{2}])=> /#.
+      by case: (GWAKEb.state_map{1}.[p{2}])=> /#.
+    auto=> /> &1 &2 + + eqsm invl a_in _ _.
+    rewrite -(eqsm (a, i){2}).
+    by case: (GWAKEb.state_map{1}.[(a, i){2}]); smt(get_setE).
+  by auto; smt().
+
 auto=> />.
-move=> &hr inv1 *. 
-split; first last.
-+ split; 2: smt(get_setE).
-  move=> a' i' j b' psk na c.
-  rewrite !get_setE //=.
-  case: (a' = a{hr}) => />; last by smt().
-  case: (i' = i{hr}) => />.
-  + case: (j = i{hr}) => />.
-    move=> neqji smj.
-    case: (inv1 a{hr} j); rewrite smj //=.
-    move=> />.
-   smt().
-  + case: (j = i{hr}) => />.
-    move=> neqji smj.
-    case: (inv1 a{hr} i'); rewrite smj //=.
-    move=> />.
-   smt().
-  smt().
-move=> a' i'.
-case ((a', i') = (a, i){hr}) => /> => [|neq_ai].
-+ apply (Red_ROM_ipending _ _ _ _ _ b{hr} ca{hr}).
-  + by rewrite !get_set_sameE.
-  + by rewrite mem_set.
-  + smt(). 
-  smt().
-apply Red_ROM_inv_neq_sm  => //.
-case (inv1 a' i') =>[
- smbj
-| r smbj
-| b c1 smbj v1 v2
-| b c1 c2 smbj v
-| r tr k smbj
-| r tr k smb
-].
-+ exact Red_ROM_undef.
-+ exact (Red_ROM_aborted _ _ _ _ _ r).
-+ apply (Red_ROM_ipending _ _ _ _ _ b c1) => //.
-  smt(mem_set).
-+ apply (Red_ROM_rpending _ _ _ _ _ b c1 c2) => //.
-  smt(mem_set).
-+ exact (Red_ROM_accepted _ _ _ _ _ r tr k).
-exact (Red_ROM_observed _ _ _ _ _ r tr k).
-qed.
-
-hoare Red_ROM_inv_send_msg2: Red_ROM(A, LRO).WAKE_O.send_msg2:
-  Red_ROM_full_inv Red_ROM.WAKE_O.state_map Red_ROM.WAKE_O.dec_map RO.m
-==>
-  Red_ROM_full_inv Red_ROM.WAKE_O.state_map Red_ROM.WAKE_O.dec_map RO.m.
-proof.
-proc; inline*.
-sp; if=> //.
-sp; match => //.
-+ auto => /> &m decn st inv1 *.
-  split; 2: smt(get_setE).
-  move=> a' i'.
-  case ((a', i') = (b, j){m}) => /> => [|neq_ai].
-  - apply (Red_ROM_aborted _ _ _ _ _ Responder).
-    by rewrite get_set_sameE. 
-  apply Red_ROM_inv_neq_sm => //.
-  exact inv1.
-seq 1 : (#pre); 1: by auto.
-case (Red_ROM.WAKE_O.bad).
-+ by rcondf ^if; auto=> />.
-auto=> />.  
-move=> &hr dm sm inv1 *.
-split; 2: smt(get_setE).
-move=> a' i'.
-case ((a', i') = (b, j){hr}) => /> => [|neq_ai].
-+ apply (Red_ROM_rpending _ _ _ _ _ a{hr} ca{hr} cb{hr}).
-  by rewrite !get_set_sameE.
-  move=> c3.
-  rewrite mem_set => />.
-  smt().
-apply Red_ROM_inv_neq_sm  => //.
-case (inv1 a' i') =>[
- smbj
-| r smbj
-| b c1 smbj v1 v2
-| b c1 c2 smbj v
-| r tr k smbj
-| r tr k smbj
-].
-+ exact Red_ROM_undef.
-+ exact (Red_ROM_aborted _ _ _ _ _ r).
-+ apply (Red_ROM_ipending _ _ _ _ _ b c1) => //.
-  smt(mem_set).
-+ apply (Red_ROM_rpending _ _ _ _ _ b c1 c2) => //.
-  smt(mem_set).
-+ exact (Red_ROM_accepted _ _ _ _ _ r tr k).
-exact (Red_ROM_observed _ _ _ _ _ r tr k).
-qed.
- 
-hoare Red_ROM_inv_send_msg3: Red_ROM(A, LRO).WAKE_O.send_msg3:
-  Red_ROM_full_inv Red_ROM.WAKE_O.state_map Red_ROM.WAKE_O.dec_map RO.m
-==>
-  Red_ROM_full_inv Red_ROM.WAKE_O.state_map Red_ROM.WAKE_O.dec_map RO.m.
-proof.
-proc; inline*.
-sp; if=> //.
-sp; match => //.
-sp; match.
-+ auto => /> &m decn st inv1 *.
-  split; 2: smt(get_setE).
-  move=> a' i'.
-  case ((a', i') = (a, i){m}) => /> => [|neq_ai].
-  - apply (Red_ROM_aborted _ _ _ _ _ Initiator).
-    by rewrite get_set_sameE. 
-  apply Red_ROM_inv_neq_sm => //.
-  exact inv1.
-seq 1 : (#pre); 1: by auto.
-case (Red_ROM.WAKE_O.bad).
-+ by rcondf ^if; auto=> />.
-sp; if=> //.
-rcondt ^if.
-+ auto=> />.
-  move=> &hr ? dm sm inv1 *.
-  have sms : (Red_ROM.WAKE_O.state_map.[(a, i)] = Some (role, IPending (b, psk, na, ca) m1)){hr} by smt().
-  by case: (inv1 a{hr} i{hr}) ; rewrite sms.
-rcondt ^if.
-+ auto=> />.
-  move=> &hr ? dm sm inv1 *.
-  have sms : (Red_ROM.WAKE_O.state_map.[(a, i)] = Some (role, IPending (b, psk, na, ca) m1)){hr} by smt().
-  rewrite mem_set /=.
-  case: (inv1 a{hr} i{hr}) ; rewrite sms //=.
-  smt().
-auto=> />.  
-move=> &hr _ dm sm inv1 inv2 inv3 inv4 inv5 inv6 inv7 aiin _ uniqcaf n _ n2 _.
-rewrite !get_set_sameE //=.
-split; first last.
-+ smt(mem_set get_setE).
-move=> a' i'.
-case ((a', i') = (a, i){hr}) => /> => [|neq_ai].
-+ apply (Red_ROM_accepted _ _ _ _ _ Initiator (m1{hr}, m2{hr}, caf{hr}) (prf (n, n2) (a{hr}, b{hr}))).
-  by rewrite !get_set_sameE.
-apply Red_ROM_inv_neq_sm  => //.
-case (inv1 a' i') =>[
- smbj
-| r smbj
-| b c1 smbj v1 v2 v3
-| b c1 c2 smbj v
-| r tr k smbj
-| r tr k smbj
-].
-+ exact Red_ROM_undef.
-+ exact (Red_ROM_aborted _ _ _ _ _ r).
-+ apply (Red_ROM_ipending _ _ _ _ _ b c1) => //.
-  + by rewrite mem_set.
-  + rewrite !mem_set v2 //=.
-    have := (inv2 a{hr} i' i{hr} b{!hr} psk{hr} na{hr} ca{hr}).
-    have smai : (Red_ROM.WAKE_O.state_map.[(a, i)] = Some (role, IPending (b{!hr}, psk, na, ca) m1)){hr} by smt().
-    case: (inv1 a{hr} i{hr}); rewrite smai //=.
-    smt().
-  move=> c2.
-  rewrite !mem_set (v3 c2) //=.
-  have := (inv2 a{hr} i' i{hr} b{!hr} psk{hr} na{hr} ca{hr}).
-  have smai : (Red_ROM.WAKE_O.state_map.[(a, i)] = Some (role, IPending (b{!hr}, psk, na, ca) m1)){hr} by smt().
-  case: (inv1 a{hr} i{hr}); rewrite smai //=.
-  smt().
-+ apply (Red_ROM_rpending _ _ _ _ _ b c1 c2) => //.
-  smt(mem_set).
-+ exact (Red_ROM_accepted _ _ _ _ _ r tr k) => //.
-exact (Red_ROM_observed _ _ _ _ _ r tr k) => //.
-qed.
-
-hoare Red_ROM_inv_send_fin: Red_ROM(A, LRO).WAKE_O.send_fin:
-  Red_ROM_full_inv Red_ROM.WAKE_O.state_map Red_ROM.WAKE_O.dec_map RO.m
-==>
-  Red_ROM_full_inv Red_ROM.WAKE_O.state_map Red_ROM.WAKE_O.dec_map RO.m.
-proof.
-proc; inline*.
-sp; if=> //.
-sp; match => //.
-sp; match.
-+ auto => /> &m decn st inv1 *.
-  split; 2: smt(get_setE).
-  move=> a' i'.
-  case ((a', i') = (b, j){m}) => /> => [|neq_ai].
-  - apply (Red_ROM_aborted _ _ _ _ _ Responder).
-    by rewrite get_set_sameE. 
-  apply Red_ROM_inv_neq_sm => //.
-  exact inv1.
-rcondf ^if.
-+ auto=> />.
-  move=> &hr dm sm inv1 *. 
-  have sms : (Red_ROM.WAKE_O.state_map.[(b, j)] = Some (role, RPending (a, psk, na, nb, ca, cb) m1 m2)){hr} by smt().
-  case: (inv1 b{hr} j{hr}) ; rewrite sms //=.
-  smt().
-rcondf ^if.
-+ auto=> />.
-  move=> &hr dm sm inv1 *.
-  have sms : (Red_ROM.WAKE_O.state_map.[(b, j)] = Some (role, RPending (a, psk, na, nb, ca, cb) m1 m2)){hr} by smt().
-  case: (inv1 b{hr} j{hr}) ; rewrite sms //=.
-  smt().
-auto=> />.  
-move=> &hr dm sm inv1 inv2 inv3 inv4 inv5 inv6 inv7 aiin n _ n2 _.
-split; 2: smt(mem_set get_setE).
-move=> a' i'.
-case ((a', i') = (b, j){hr}) => /> => [|neq_ai].
-+ apply (Red_ROM_accepted _ _ _ _ _ Responder (m1{hr}, m2{hr}, m3{hr}) (prf (oget RO.m{hr}.[msg1_data a{hr} b{hr}, ca{hr}],
-      oget RO.m{hr}.[msg2_data a{hr} b{hr} ca{hr}, cb{hr}])
-     (a{hr}, b{hr}))).
-  by rewrite !get_set_sameE.
-apply Red_ROM_inv_neq_sm  => //.
-exact inv1.
-qed.
-
-hoare Red_ROM_inv_rev_skey: Red_ROM(A, LRO).WAKE_O.rev_skey:
-  Red_ROM_full_inv Red_ROM.WAKE_O.state_map Red_ROM.WAKE_O.dec_map RO.m
-==>
-  Red_ROM_full_inv Red_ROM.WAKE_O.state_map Red_ROM.WAKE_O.dec_map RO.m.
-proof.
-proc.
-sp; if=> //.
-sp; match => //; 2: by auto.
-sp; if=> //.
-wp 2.
-conseq (: _ ==> true); last by auto.
-auto => /> &m st inv1 inv2 inv3 inv4 inv5 inv6 inv7 aiin _ k.
-split; 2: smt(get_setE).
-move=> a' i'.
-case ((a', i') = (a, i){m}) => [eq_ai|neq_ai].
-- apply (Red_ROM_observed _ _ _ _ _ role{m} trace{m} k).
-  smt(get_setE).
-apply Red_ROM_inv_neq_sm => //.
-exact inv1.
-qed.
-
-hoare Red_ROM_inv_test: Red_ROM(A, LRO).WAKE_O.test:
-  Red_ROM_full_inv Red_ROM.WAKE_O.state_map Red_ROM.WAKE_O.dec_map RO.m
-==>
-  Red_ROM_full_inv Red_ROM.WAKE_O.state_map Red_ROM.WAKE_O.dec_map RO.m.
-proof.
-proc.
-sp; if=> //.
-sp; match => //; 2: by auto.
-sp; if=> //.
-wp 2.
-conseq (: _ ==> true); last by auto.
-auto => /> &m st inv1 inv2 inv3 inv4 inv5 inv6 inv7 aiin _ k.
-split; 2: smt(get_setE).
-move=> a' i'.
-case ((a', i') = (a, i){m}) => [eq_ai|neq_ai].
-- apply (Red_ROM_observed _ _ _ _ _ role{m} trace{m} k).
-  smt(get_setE).
-apply Red_ROM_inv_neq_sm => //.
-exact inv1.
+split; 1: smt(emptyE).
+move=> a i. 
+apply GWAKE0_undef.
+smt(emptyE).
 qed.
 
 (* ------------------------------------------------------------------------------------------ *)
+(* Step 1: Apply the AEAD assumption. *)
 
-local clone import DProd.ProdSampling with
-  type t1 <- nonce,
-  type t2 <- nonce
-proof *.
-
-lemma Step4 &m: Pr[E_GWAKE(Game4, A).run() @ &m : res] = Pr[E_GWAKE(Game5, A).run() @ &m : res].
-byequiv => //.
-proc*.
-transitivity* {1} { r <@ MainD(Red_ROM(A), RO).distinguish(); } => //.
-+ smt().
-
-+ inline*.
+lemma Step1 &m:
+    `|Pr[E_GWAKE(Game1, A).run() @ &m : res] - Pr[E_GWAKE(Game2, A).run() @ &m : res]|
+  = 
+    `|Pr[E_GAEAD(GAEAD0, Red_AEAD(A)).run() @ &m : res] - Pr[E_GAEAD(GAEAD1, Red_AEAD(A)).run() @ &m : res]|.
+proof.
+do! congr.
++ byequiv => //.
+  proc; inline*.
   wp.
-  call (: ={state_map, psk_map, bad}(Game4, Red_ROM.WAKE_O)
-       /\ (forall h, h \in Game4.dec_map{1} <=> h \in Red_ROM.WAKE_O.dec_map{2})
-       /\ (forall c ad n, (exists pk, Game4.dec_map{1}.[(pk, ad, c)] = Some n) <=> RO.m{2}.[(ad, c)] = Some n)
-       /\ (forall a b ca cb, ((a, b), msg2_data a b ca, cb) \in Game4.dec_map => ((a, b), msg1_data a b, ca) \in Game4.dec_map){1}
-       /\ (forall a b ca cb caf, ((a, b), msg3_data a b ca cb, caf) \in Game4.dec_map => ((a, b), msg2_data a b ca, cb) \in Game4.dec_map){1}
-  ) => //.
+  call (:
+        ={psk_map}(Game1, GAEADb)
+     /\ ={state_map}(Game1, Red_AEAD.WAKE_O)
+     /\ (forall a i, Game1_inv Game1.state_map Game1.psk_map a i){1}
+  )=> //.
 
-  - by proc; sp; if; auto.
+  - conseq (: ={res}
+         /\ ={psk_map}(Game1, GAEADb)
+         /\ ={state_map}(Game1, Red_AEAD.WAKE_O)
+    ) Game1_inv_gen_pskey _ => //.
+    by proc; if; auto.
 
-  - proc; inline*.
+  - conseq (: ={res}
+         /\ ={psk_map}(Game1, GAEADb)
+         /\ ={state_map}(Game1, Red_AEAD.WAKE_O)
+    ) Game1_inv_send_msg1 _ => //.
+    proc; inline.
     sp; if=> //.
-    seq 1 1 : (#pre /\ ={ca}); 1: by auto.
+    by match Some {2} ^match; auto; smt().
+
+  - conseq (: ={res}
+         /\ ={psk_map}(Game1, GAEADb)
+         /\ ={state_map}(Game1, Red_AEAD.WAKE_O)
+    ) Game1_inv_send_msg2 _ => //.
+    proc; inline.
     sp; if=> //.
+    match Some {2} ^match.
+    + auto; smt().
+    sp; match =.
     + smt().
-    + rcondt {2} ^if; 1: by auto=> /#. 
-      auto=> />.
-      smt(get_setE).
+    + by auto. 
+    move=> na.
+    by match Some {2} ^match; auto; smt().
+
+  - conseq (: ={res}
+         /\ ={psk_map}(Game1, GAEADb)
+         /\ ={state_map}(Game1, Red_AEAD.WAKE_O)
+    ) Game1_inv_send_msg3 _ => //.
+    proc; inline.
+    sp; if=> //.
+    sp; match = => //. 
+    + smt().
+    move=> st m1.
+    match Some {2} ^match.
+    + auto=> />.
+      move=> &hr smr sml invl ai_in.
+      by case: (invl a{m0} i{m0})=> /#.
+    sp; match =.
+    + by auto=> /#. 
+    + by auto=> /#.
+    move=> nb.
+    match Some {2} ^match.
+    + auto=> /> &1 decl decr smr sml invl ai_in ok _.
+      by case: (invl a{m0} i{m0})=> /#.
     by auto=> /#.
-  
-   - proc; inline*.
-     sp; if=> //. 
-     match; 1,2: smt().
-     + by auto=> />.
-     move=> nal nar.
-     seq 1 1 : (#pre /\ ={cb}); 1: by auto.
-     sp; if=> //.
-     + smt().
-     + rcondt {2} ^if; 1: by auto=> /#. 
-       auto=> />.
-       smt(get_setE).
-     auto=> />.
-     smt(). 
 
-   - proc; inline*.
-     sp; if=> //. 
-     sp; match = => //.
-     + smt().
-     move=> s m1.
-     sp; match; 1,2: smt().
-     + by auto=> />.
-     move=> nbl nbr.
-     seq 1 1 : (#pre /\ ={caf}); 1: by auto.
-     case (Game4.bad{1}).
-     + rcondf {1} ^if; 1: by auto=> />.
-       rcondf {2} ^if; 1: by auto=> />.
-       by auto=> />.
-     sp; if=> //.
-     + smt().
-     + rcondt {2} ^if; 1: by auto=> /#.
-       rcondf {2} ^if.
-       + auto=> />.
-         smt(mem_set).
-       rcondf {2} ^if.
-       + auto=> />.
-         smt(mem_set).
-       swap {2} ^r1<$ @ ^x<-.
-       seq 1 1 : (#pre /\ ok{1} = r1{2}); 1: by auto => />.
-       auto=> />.
-       + smt(get_setE).
-    auto=> />.
-    smt().
-  
-   - proc; inline*.
-     sp; if=> //. 
-     sp; match = => //.
-     + smt().
-     move=> s m1 m2.
-     sp; match; 1,2: smt().
-     + by auto=> />.
-     move=> nokl nokr.
-     rcondf {2} ^if; 1: by auto=> /#.
-     rcondf {2} ^if; 1: by auto=> /#.
-     auto=> />.
-     smt(get_setE).
-  
-   - by sim />.
-   
-   - by sim />.
+  - conseq (: ={res}
+         /\ ={psk_map}(Game1, GAEADb)
+         /\ ={state_map}(Game1, Red_AEAD.WAKE_O)
+    ) Game1_inv_send_fin _ => //.
+    proc; inline.
+    sp; if=> //.
+    sp; match = => //.
+    + smt().
+    move=> st m1 m2.
+    match Some {2} ^match.
+    + auto=> />. 
+      move=> &hr smr sml invl bj_in.
+      by case: (invl b{m0} j{m0})=> /#.
+    by sp; match =; auto=> /#.
 
-   auto=> />.
-   smt(emptyE).
+  - conseq (: ={res}
+         /\ ={psk_map}(Game1, GAEADb)
+         /\ ={state_map}(Game1, Red_AEAD.WAKE_O)
+    ) Game1_inv_rev_skey _ => //.
+    by sim. 
+
+  - conseq (: ={res}
+         /\ ={psk_map}(Game1, GAEADb)
+         /\ ={state_map}(Game1, Red_AEAD.WAKE_O)
+    ) Game1_inv_test _ => //.
+    by sim. 
   
-have ll : forall (c : msg_data * ctxt), is_lossless dnonce by move=> _; exact dnonce_ll.
-rewrite equiv [{1} 1 (FullEager.RO_LRO (Red_ROM(A)) ll)].
-inline*.
-wp; call (: 
-  ={state_map, psk_map, bad, dec_map}(Red_ROM.WAKE_O, Game5)
-  /\ (forall a b ca cb caf, ((a, b), msg3_data a b ca cb, caf) \in Red_ROM.WAKE_O.dec_map{1} =>
-       oget Game5.prfkey_map{2}.[caf] = (oget RO.m{1}.[(msg1_data a b, ca)], oget RO.m{1}.[(msg2_data a b ca, cb)]))
-  /\ (Red_ROM_full_inv Red_ROM.WAKE_O.state_map Red_ROM.WAKE_O.dec_map RO.m){1}
-) => //.
-
-- by sim />.
-
-- conseq (: ={res}
-  /\ ={state_map, psk_map, bad, dec_map}(Red_ROM.WAKE_O, Game5)
-  /\ (forall a b ca cb caf, ((a, b), msg3_data a b ca cb, caf) \in Red_ROM.WAKE_O.dec_map{1} =>
-       oget Game5.prfkey_map{2}.[caf] = (oget RO.m{1}.[(msg1_data a b, ca)], oget RO.m{1}.[(msg2_data a b ca, cb)]))
-  ) Red_ROM_inv_send_msg1 _ => //.
-  proc; inline*.
-  sp; if=> //.
-  seq 1 1 : (#pre /\ ={ca}); 1: by auto.
-  case (Red_ROM.WAKE_O.bad{1}).
-  + rcondf {1} ^if; 1: by auto=> />.
-    rcondf {2} ^if; 1: by auto=> />.
-    auto=> />.
-  sp 1 1; if=> //.
   auto=> />.
-  smt(get_setE).
+  move=> a i.
+  exact /Game1_undef/emptyE.
+
+byequiv => //.
+proc; inline*.
+wp.
+call (:
+      ={psk_map}(Game2, GAEADb)
+      /\ ={state_map}(Game2, Red_AEAD.WAKE_O)
+      /\ Game2.dec_map{1} = GAEAD1.ctxts{2}
+      /\ (forall a i, Game1_inv Game2.state_map Game2.psk_map a i){1}
+).
+- conseq (: ={res}
+       /\ ={psk_map}(Game2, GAEADb)
+       /\ ={state_map}(Game2, Red_AEAD.WAKE_O)
+       /\ Game2.dec_map{1} = GAEAD1.ctxts{2}
+  ) Game2_inv_gen_pskey _ => //.
+  proc.
+  by if; auto.
 
 - conseq (: ={res}
-  /\ ={state_map, psk_map, bad, dec_map}(Red_ROM.WAKE_O, Game5)
-  /\ (forall a b ca cb caf, ((a, b), msg3_data a b ca cb, caf) \in Red_ROM.WAKE_O.dec_map{1} =>
-       oget Game5.prfkey_map{2}.[caf] = (oget RO.m{1}.[(msg1_data a b, ca)], oget RO.m{1}.[(msg2_data a b ca, cb)]))
-  ) Red_ROM_inv_send_msg2 _ => //.
-  proc; inline*.
+       /\ ={psk_map}(Game2, GAEADb)
+       /\ ={state_map}(Game2, Red_AEAD.WAKE_O)
+       /\ Game2.dec_map{1} = GAEAD1.ctxts{2}
+  ) Game2_inv_send_msg1 _ => //.
+  proc; inline.
   sp; if=> //.
+  rcondt{2} ^if; 1: by auto.
+  swap {2} ^c<$ @ ^na<$.
+  by auto.
+
+- conseq (: ={res}
+       /\ ={psk_map}(Game2, GAEADb)
+       /\ ={state_map}(Game2, Red_AEAD.WAKE_O)
+       /\ Game2.dec_map{1} = GAEAD1.ctxts{2}
+  ) Game2_inv_send_msg2 _ => //.
+  proc; inline.
+  sp; if=> //.
+  rcondt {2} 5; 1: by auto.
   sp; match = => //.
-  + by auto=> />.
+  + by auto.
   move=> na.
-  seq 1 1 : (#pre /\ ={cb}); 1: by auto.
-  case (Red_ROM.WAKE_O.bad{1}).
-  + rcondf {1} ^if; 1: by auto=> />.
-    rcondf {2} ^if; 1: by auto=> />.
-    auto=> />.
-  sp 1 1; if=> //.
-  auto=> />.
-  smt(get_setE). 
+  rcondt {2} ^if; 1: by auto.
+  swap {2} ^c0<$ @ ^nb<$.
+  by auto.
 
 - conseq (: ={res}
-  /\ ={state_map, psk_map, bad, dec_map}(Red_ROM.WAKE_O, Game5)
-  /\ (forall a b ca cb caf, ((a, b), msg3_data a b ca cb, caf) \in Red_ROM.WAKE_O.dec_map{1} =>
-       oget Game5.prfkey_map{2}.[caf] = (oget RO.m{1}.[(msg1_data a b, ca)], oget RO.m{1}.[(msg2_data a b ca, cb)]))
-  ) Red_ROM_inv_send_msg3 _ => //.
-  proc; inline*.
+       /\ ={psk_map}(Game2, GAEADb)
+       /\ ={state_map}(Game2, Red_AEAD.WAKE_O)
+       /\ Game2.dec_map{1} = GAEAD1.ctxts{2}
+  ) Game2_inv_send_msg3 _ => //.
+  proc; inline.
   sp; if=> //.
   sp; match = => //.
   + smt().
-  move=> s m1.
-  sp; match = => //.
+  move=> st m1.
+  rcondt {2} ^if.
+  + auto=> />.
+    move=> &hr smr sml invl ai_in.
+    by case: (invl a{m0} i{m0})=> /#.
+  sp; match =.
+  + by auto.
   + by auto.
   move=> nb.
-  seq 1 1 : (#pre /\ ={caf}); 1: by auto.
-  case (Red_ROM.WAKE_O.bad{1}).
-  + rcondf {1} ^if; 1: by auto=> />.
-    rcondf {2} ^if; 1: by auto=> />.
-    auto=> />.
-  sp 1 1; if=> //.
-  rcondt {1} ^if.
+  rcondt {2} ^if.
   + auto=> />.
-    move=> &hr ? dm _ sm _ inv1 invl1 *. 
-    have sms : (Game5.state_map.[(a, i)] = Some (role, IPending (b, psk, na, ca) m1)){m0} by smt().
-    by case: (invl1 a{m0} i{m0}) ; rewrite sms.
-  rcondt {1} ^if.
-  + auto=> />.
-    move=> &hr ? dm _ sm _ inv1 invl1 *.
-    have sms : (Game5.state_map.[(a, i)] = Some (role, IPending (b, psk, na, ca) m1)){m0} by smt().
-    rewrite mem_set //=.
-    case: (invl1 a{m0} i{m0}) ; rewrite sms //=.
-    smt().
-  outline {2} [3] (na, ok) <@ S.sample. 
-  wp; rewrite equiv [{2} 3 sample_sample2].
-  inline*.
-  auto=> />.
-  move=> &1 &2 ? dm _ sm _ inv1 invl1 invl2 invl3 invl4 invl5 invl6 invl7 *.
-  rewrite get_set_sameE //=.
-  split; 1: smt(get_setE).
-  move=> a' b' ca' cb' caf'. 
-  rewrite mem_set => />.
-  case; 2: smt(get_setE).
-  have smai : (Game5.state_map.[(a, i)] = Some (role, IPending (b, psk, na, ca) m1)){2} by smt().
-  case: (invl1 a{2} i{2}); rewrite smai //=.
-  smt(get_setE).
+    move=> &hr decl decr smr sml invl ai_in ok _.
+    by case: (invl a{m0} i{m0})=> /#.
+  swap {2} ^c0<$ @ ^ok<$.
+  by auto.
 
 - conseq (: ={res}
-  /\ ={state_map, psk_map, bad, dec_map}(Red_ROM.WAKE_O, Game5)
-  /\ (forall a b ca cb caf, ((a, b), msg3_data a b ca cb, caf) \in Red_ROM.WAKE_O.dec_map{1} =>
-       oget Game5.prfkey_map{2}.[caf] = (oget RO.m{1}.[(msg1_data a b, ca)], oget RO.m{1}.[(msg2_data a b ca, cb)]))
-  ) Red_ROM_inv_send_fin _ => //.
-- proc; inline*.
+       /\ ={psk_map}(Game2, GAEADb)
+       /\ ={state_map}(Game2, Red_AEAD.WAKE_O)
+       /\ Game2.dec_map{1} = GAEAD1.ctxts{2}
+  ) Game2_inv_send_fin _ => //.
+  proc; inline.
   sp; if=> //.
   sp; match = => //.
   + smt().
-  move=> s m1 m2.
-  sp; match = => //.
-  + by auto.
-  move=> nok.
-  rcondf {1} ^if.
+  move=> st m1 m2.
+  rcondt {2} 6.
   + auto=> />.
-    move=> &hr dm _ sm _ inv1 inl *.
-    have sms : (Game5.state_map.[(b, j)] = Some (role, RPending (a, psk, na, nb, ca, cb) m1 m2)){m0} by smt().
-    case: (inl b{m0} j{m0}) ; rewrite sms //=.
-    smt().
-  rcondf {1} ^if.
-  + auto=> />.
-    move=> &hr dm _ sm _ inv1 inl *.
-    have sms : (Game5.state_map.[(b, j)] = Some (role, RPending (a, psk, na, nb, ca, cb) m1 m2)){m0} by smt().
-    case: (inl b{m0} j{m0}) ; rewrite sms //=.
-    smt().
-  auto=> />.
-  smt().
+    move=> &hr smr sml invl ai_in.
+    by case: (invl b{m0} j{m0})=> /#.
+  by sp; match =; auto.
 
 - conseq (: ={res}
-  /\ ={state_map, psk_map, bad, dec_map}(Red_ROM.WAKE_O, Game5)
-  /\ (forall a b ca cb caf, ((a, b), msg3_data a b ca cb, caf) \in Red_ROM.WAKE_O.dec_map{1} =>
-       oget Game5.prfkey_map{2}.[caf] = (oget RO.m{1}.[(msg1_data a b, ca)], oget RO.m{1}.[(msg2_data a b ca, cb)]))
-  ) Red_ROM_inv_rev_skey _ => //.
-  by sim />.
+       /\ ={psk_map}(Game2, GAEADb)
+       /\ ={state_map}(Game2, Red_AEAD.WAKE_O)
+       /\ Game2.dec_map{1} = GAEAD1.ctxts{2}
+  ) Game2_inv_rev_skey _ => //.
+  by sim.
 
 - conseq (: ={res}
-  /\ ={state_map, psk_map, bad, dec_map}(Red_ROM.WAKE_O, Game5)
-  /\ (forall a b ca cb caf, ((a, b), msg3_data a b ca cb, caf) \in Red_ROM.WAKE_O.dec_map{1} =>
-       oget Game5.prfkey_map{2}.[caf] = (oget RO.m{1}.[(msg1_data a b, ca)], oget RO.m{1}.[(msg2_data a b ca, cb)]))
-  ) Red_ROM_inv_test _ => //.
-  by sim />.
+       /\ ={psk_map}(Game2, GAEADb)
+       /\ ={state_map}(Game2, Red_AEAD.WAKE_O)
+       /\ Game2.dec_map{1} = GAEAD1.ctxts{2}
+  ) Game2_inv_test _ => //.
+  by sim.
 
-auto => />.
-smt(emptyE Red_ROM_undef).
+auto=> /> a i.
+exact /Game1_undef/emptyE.
 qed.
+
+(* ------------------------------------------------------------------------------------------ *)
+(* Step 2: Remove collisions of all produced ciphertexts. *)
+
+lemma Step2 &m: `| Pr[E_GWAKE(Game2, A).run() @ &m : res] - Pr[E_GWAKE(Game3, A).run() @ &m : res] | <= Pr[E_GWAKE(Game3, A).run() @ &m : Game3.bad].
+proof.
+byequiv (: _ ==> _) : Game2.bad => //; first last.
++ move=> &1 &2.
+  by case: (Game3.bad{2}).
+proc; inline*.
+call (: Game3.bad, ={bad, psk_map, state_map, dec_map}(Game2, Game3), ={bad}(Game2, Game3)) => //.
++ exact A_ll.
+
++ by proc; inline*; auto; if; auto.
++ move=> &2 ->.
+  proc; sp; if; auto.
+  by rewrite dpskey_ll.  
++ move=> &1.
+  proc; sp; if; auto.
+  by rewrite dpskey_ll. 
+ 
++ proc.
+  sp; if=> //.
+  seq 1 1: (#pre /\ ={ca}); 1: by auto.
+  sp 1 1.
+  by if{2}; auto=> />.
++ move=> &2 ->.
+  proc; sp; if=> //; auto.
+  by rewrite dnonce_ll dctxt_ll.
++ move=> &1.
+  proc; sp; if=> //.
+  rcondf ^if; auto=> />.
+  by rewrite dctxt_ll.
+
++ proc.
+  sp; if=> //.
+  match = => //.
+  + by auto.
+  move=> na.
+  seq 1 1: (#pre /\ ={cb}); 1: by auto.
+  sp 0 1.
+  by if{2}; auto=> />.
++ move=> &2 ->.
+  proc; sp; if=> //; match =; auto.
+  by rewrite dnonce_ll dctxt_ll.
++ move=> &1.
+  proc; sp; if=> //; match =; auto.
+  rcondf ^if; auto=> />.
+  by rewrite dctxt_ll.
+
++ proc.
+  sp; if=> //.
+  sp; match = => //.
+  - smt().
+  move => s m1.
+  sp; match = => //.
+  + by auto.  
+  move=> nb.
+  seq 1 1: (#pre /\ ={caf}); 1: by auto.
+  sp 0 1.
+  by if{2}; auto=> />.
++ move=> &2 ->.
+  proc; sp; if=> //; sp; match =; auto; sp; match =; auto.
+  by rewrite dnonce_ll dctxt_ll.
++ move=> &1.
+  proc; sp; if=> //; sp; match =; auto; sp; match =; auto.
+  rcondf ^if; auto=> />.
+  by rewrite dctxt_ll.
+
++ proc.
+  sp; if=> //.
+  sp; match =; auto; smt(). 
++ move=> &2 ->.
+  proc; sp; if=> //; sp; match =; auto; smt().
++ move=> &1.
+  proc; sp; if=> //; sp; match =; auto; smt().
+
++ proc.
+  sp; if=> //.
+  sp; match =; auto; smt(). 
++ move=> &2 ->.
+  proc; sp; if=> //; sp; match =; auto; smt().
++ move=> &1.
+  proc; sp; if=> //; sp; match =; auto; smt().
+
+
++ proc.
+  sp; if=> //.
+  sp; match =; auto; smt(). 
++ move=> &2 ->.
+  proc; sp; if=> //; sp; match =; auto; smt().
++ move=> &1.
+  proc; sp; if=> //; sp; match =; auto; smt().
+auto=> />.
+move=> rl rr al bl dl pl sl ar br dr pr sr. 
+by case : (!br) => />.
+qed.
+
+(* ------------------------------------------------------------------------------------------ *)
+(* Step 3: No longer store nonces in the state, just retrieve from the dec_map. *)
 
 local op clear_nonces (s : instance_state) =
 match s with
@@ -1373,496 +1191,274 @@ move=> a i.
 exact /Game3_undef/emptyE.
 qed.
 
-lemma Step2 &m: `| Pr[E_GWAKE(Game2, A).run() @ &m : res] - Pr[E_GWAKE(Game3, A).run() @ &m : res] | <= Pr[E_GWAKE(Game3, A).run() @ &m : Game3.bad].
-proof.
-byequiv (: _ ==> _) : Game2.bad => //; first last.
-+ move=> &1 &2.
-  by case: (Game3.bad{2}).
-proc; inline*.
-call (: Game3.bad, ={bad, psk_map, state_map, dec_map}(Game2, Game3), ={bad}(Game2, Game3)) => //.
-+ exact A_ll.
+(* ------------------------------------------------------------------------------------------ *)
+(* Step 4: Delay the sampling of na and nb until msg3, sampling them together. *)
 
-+ by proc; inline*; auto; if; auto.
-+ move=> &2 ->.
-  proc; sp; if; auto.
-  by rewrite dpskey_ll.  
-+ move=> &1.
-  proc; sp; if; auto.
-  by rewrite dpskey_ll. 
- 
-+ proc.
-  sp; if=> //.
-  seq 1 1: (#pre /\ ={ca}); 1: by auto.
-  sp 1 1.
-  by if{2}; auto=> />.
-+ move=> &2 ->.
-  proc; sp; if=> //; auto.
-  by rewrite dnonce_ll dctxt_ll.
-+ move=> &1.
-  proc; sp; if=> //.
-  rcondf ^if; auto=> />.
-  by rewrite dctxt_ll.
+local clone import DProd.ProdSampling with
+  type t1 <- nonce,
+  type t2 <- nonce
+proof *.
 
-+ proc.
-  sp; if=> //.
-  match = => //.
-  + by auto.
-  move=> na.
-  seq 1 1: (#pre /\ ={cb}); 1: by auto.
-  sp 0 1.
-  by if{2}; auto=> />.
-+ move=> &2 ->.
-  proc; sp; if=> //; match =; auto.
-  by rewrite dnonce_ll dctxt_ll.
-+ move=> &1.
-  proc; sp; if=> //; match =; auto.
-  rcondf ^if; auto=> />.
-  by rewrite dctxt_ll.
-
-+ proc.
-  sp; if=> //.
-  sp; match = => //.
-  - smt().
-  move => s m1.
-  sp; match = => //.
-  + by auto.  
-  move=> nb.
-  seq 1 1: (#pre /\ ={caf}); 1: by auto.
-  sp 0 1.
-  by if{2}; auto=> />.
-+ move=> &2 ->.
-  proc; sp; if=> //; sp; match =; auto; sp; match =; auto.
-  by rewrite dnonce_ll dctxt_ll.
-+ move=> &1.
-  proc; sp; if=> //; sp; match =; auto; sp; match =; auto.
-  rcondf ^if; auto=> />.
-  by rewrite dctxt_ll.
-
-+ proc.
-  sp; if=> //.
-  sp; match =; auto; smt(). 
-+ move=> &2 ->.
-  proc; sp; if=> //; sp; match =; auto; smt().
-+ move=> &1.
-  proc; sp; if=> //; sp; match =; auto; smt().
-
-+ proc.
-  sp; if=> //.
-  sp; match =; auto; smt(). 
-+ move=> &2 ->.
-  proc; sp; if=> //; sp; match =; auto; smt().
-+ move=> &1.
-  proc; sp; if=> //; sp; match =; auto; smt().
-
-
-+ proc.
-  sp; if=> //.
-  sp; match =; auto; smt(). 
-+ move=> &2 ->.
-  proc; sp; if=> //; sp; match =; auto; smt().
-+ move=> &1.
-  proc; sp; if=> //; sp; match =; auto; smt().
-auto=> />.
-move=> rl rr al bl dl pl sl ar br dr pr sr. 
-by case : (!br) => />.
-qed.
-
-local op clear_psk (s : instance_state) =
-match s with
-| IPending st m1 => 
-  let (id, psk, na, ca) = st in IPending (id, witness, na, ca) m1 
-| RPending st m1 m2 => 
-  let (id, psk, na, nb, ca, cb) = st in RPending (id, witness, na, nb, ca, cb) m1 m2 
-| Accepted _ _ => s
-| Observed _ _ => s
-| Aborted => s
-end.
-
-local lemma eq_partners h tr r sml smr: 
-  (forall h, omap (fun (v: role * instance_state) => let (r, s) = v in (r, clear_psk s)) sml.[h] = smr.[h]) =>
-get_partners h tr r sml = get_partners h tr r smr.
-proof.
-move=> eqsm.
-rewrite /get_partners.
-congr.
-apply fmap_eqP => h'.
-rewrite !filterE -(eqsm h') /=. 
-case: (sml.[h'])=> //=.
-by move=> [r' []] // [] /= /#.
-qed.
-
-local lemma eq_obs_partners h sml smr: 
-  (forall h, omap (fun (v: role * instance_state) => let (r, s) = v in (r, clear_psk s)) sml.[h] = smr.[h]) =>
-get_observed_partners h sml = get_observed_partners h smr.
-proof.
-move=> eqsm.
-rewrite /get_observed_partners.
-congr.
-+ rewrite fun_ext => bj.
-  rewrite -(eqsm bj) //=.
-  case: (sml.[bj])=> //.
-  by move=> [r' []] // [].
-rewrite -(eq_partners _ _ _ sml smr eqsm). 
-rewrite -(eqsm h) /s /r //=.
-case: (sml.[h])=> //.
-by move=> [r' []] // [].
-qed.
-
-lemma Step0 &m:
-    Pr[E_GWAKE(GWAKE0(NSL), A).run() @ &m : res] = Pr[E_GWAKE(Game1, A).run() @ &m : res].
-proof.
+lemma Step4 &m: Pr[E_GWAKE(Game4, A).run() @ &m : res] = Pr[E_GWAKE(Game5, A).run() @ &m : res].
 byequiv => //.
-proc; inline*.
-call (:
-    ={psk_map}(GWAKEb, Game1)
-/\ (forall h, omap (fun v => let (r, s) = v in (r, clear_psk s)) GWAKEb.state_map.[h]{1} = Game1.state_map.[h]{2})
-/\ (forall a i, GWAKE0_inv GWAKEb.state_map GWAKEb.psk_map a i){1}
-).
-- conseq (: ={res}
-          /\ ={psk_map}(GWAKEb, Game1)
-          /\ (forall h, omap (fun v => let (r, s) = v in (r, clear_psk s)) GWAKEb.state_map.[h]{1} = Game1.state_map.[h]{2})
-  ) GWAKE0_inv_gen_pskey _ => //.
-  proc.
-  by if; auto.
+proc*.
+transitivity* {1} { r <@ MainD(Red_ROM(A), RO).distinguish(); } => //.
++ smt().
 
-- conseq (: ={res}
-          /\ ={psk_map}(GWAKEb, Game1)
-          /\ (forall h, omap (fun v => let (r, s) = v in (r, clear_psk s)) GWAKEb.state_map.[h]{1} = Game1.state_map.[h]{2})
-     ) GWAKE0_inv_send_msg1 _ => //.
-  proc; inline.
-  sp; if=> //.
-  + smt().
-  auto=> />.
-  smt(get_setE).
-
-- conseq (: ={res}
-          /\ ={psk_map}(GWAKEb, Game1)
-          /\ (forall h, omap (fun v => let (r, s) = v in (r, clear_psk s)) GWAKEb.state_map.[h]{1} = Game1.state_map.[h]{2})
-     ) GWAKE0_inv_send_msg2 _ => //.
-  proc; inline.
-  sp; if=> //.
-  + smt().
-  sp; match =.
-  + smt().
-  + auto=> />.
-    smt(get_setE).
-  move=> na.
-  by match Some {1} ^match; auto; smt(get_setE).
-
-- conseq (: ={res}
-          /\ ={psk_map}(GWAKEb, Game1)
-          /\ (forall h, omap (fun v => let (r, s) = v in (r, clear_psk s)) GWAKEb.state_map.[h]{1} = Game1.state_map.[h]{2})
-     ) GWAKE0_inv_send_msg3 _ => //.
-  proc; inline.
-  sp; if=> //.
-  + smt().
-  sp; match; 1..5: smt(); 2..5: by auto.
-  move=> sil m1l sir m1r.
-  sp; match =.
-  + auto=> />.
-    move=> &1 &2 smr sml inv_sm invl ai_in.
-    case: (invl a{2} i{2})=> /#.
-  + match None {1} ^match; auto; smt(get_setE).
-  move=> nb.
-  match Some {1} ^match.
-  + auto; smt(get_setE).
-  auto=> />.
-  move=> &1 &2 + + + sml + invl.
-  case: (invl a{2} i{2}); 1,2,4,5,6: smt().
-  smt(get_setE).
-
-- conseq (: ={res}
-          /\ ={psk_map}(GWAKEb, Game1)
-          /\ (forall h, omap (fun v => let (r, s) = v in (r, clear_psk s)) GWAKEb.state_map.[h]{1} = Game1.state_map.[h]{2})
-     ) GWAKE0_inv_send_fin _ => //.
-  proc; inline.
-  sp; if=> //.
-  + smt().
-  sp; match; 1..5: smt(); 1,3,4,5: by auto.
-  move=> sil m1l m2l sir m1r m2r.
-  sp; match =.
-  + auto=> />. 
-    move=> &1 &2 smr sml inv_sm invl bj_in.
-    case: (invl b{2} j{2})=> /#.
-  + match None {1} ^match; auto; smt(get_setE).
-  move=> nb.
-  match Some {1} ^match.
-  + auto; smt(get_setE).
-  auto=> />.
-  move=> &1 &2 + + + sml + invl.
-  case: (invl b{2} j{2}); 1,2,3,5,6: smt().
-  smt(get_setE).
-
-- conseq (: ={res}
-          /\ ={psk_map}(GWAKEb, Game1)
-          /\ (forall h, omap (fun v => let (r, s) = v in (r, clear_psk s)) GWAKEb.state_map.[h]{1} = Game1.state_map.[h]{2})
-     ) GWAKE0_inv_rev_skey _ => //.
-  proc; inline. 
-  sp; if=> //.
-  + smt().
-  sp; match; 1..5: smt(); 1,2,5: by auto.
-  + move=> tr k tr' k'.
-    sp ^if & -1 ^if & -1; if=> //.
-    + smt(eq_partners).
-    sp ^if & -1 ^if & -1; if.
-    + move=> /> &1 &2 smr sml eqsm.
-      by rewrite (eq_obs_partners (a, i){2} GWAKEb.state_map{1} Game1.state_map{2}).
-    + seq 1 1 : (={ps, p} /\ #pre).
-      + auto=> /> &1 &2 smr sml eqsm.
-        by rewrite (eq_obs_partners (a, i){2} GWAKEb.state_map{1} Game1.state_map{2}).
-      wp 2 2.
-      conseq (: _ ==> ={k, role} /\ tr = tr').
-      + move=> /> &1 &2 _ + + eqsm invl a_in _ _.
-        rewrite -(eqsm (a, i){2}).
-        by case: (GWAKEb.state_map{1}.[(a, i){2}]); smt(get_setE).
-      auto=> /> &1 &2 + + + eqsm invl a_in _ _.
-      rewrite -(eqsm (a, i){2}) -(eqsm p{2}).
-      case: (GWAKEb.state_map{1}.[(a, i){2}])=> />.
-      + by case: (GWAKEb.state_map{1}.[p{2}])=> /#.
-      by case: (GWAKEb.state_map{1}.[p{2}])=> /#.
-    auto=> /> &1 &2 + + eqsm invl a_in _ _.
-    rewrite -(eqsm (a, i){2}).
-    by case: (GWAKEb.state_map{1}.[(a, i){2}]); smt(get_setE).
-  by auto; smt().
-
-- conseq (: ={res}
-          /\ ={psk_map}(GWAKEb, Game1)
-          /\ (forall h, omap (fun v => let (r, s) = v in (r, clear_psk s)) GWAKEb.state_map.[h]{1} = Game1.state_map.[h]{2})
-     ) GWAKE0_inv_test _ => //.
-  proc; inline. 
-  sp; if=> //.
-  + smt().
-  sp; match; 1..5: smt(); 1,2,5: by auto.
-  + move=> tr k tr' k'.
-    sp ^if & -1 ^if & -1; if=> //.
-    + smt(eq_partners).
-    sp ^if & -1 ^if & -1; if.
-    + move=> /> &1 &2 smr sml eqsm.
-      by rewrite (eq_obs_partners (a, i){2} GWAKEb.state_map{1} Game1.state_map{2}).
-    + seq 1 1 : (={ps, p} /\ #pre).
-      + auto=> /> &1 &2 smr sml eqsm.
-        by rewrite (eq_obs_partners (a, i){2} GWAKEb.state_map{1} Game1.state_map{2}).
-      wp 2 2.
-      conseq (: _ ==> ={k, role} /\ tr = tr').
-      + move=> /> &1 &2 _ + + eqsm invl a_in _ _.
-        rewrite -(eqsm (a, i){2}).
-        by case: (GWAKEb.state_map{1}.[(a, i){2}]); smt(get_setE).
-      auto=> /> &1 &2 + + + eqsm invl a_in _ _.
-      rewrite -(eqsm (a, i){2}) -(eqsm p{2}).
-      case: (GWAKEb.state_map{1}.[(a, i){2}])=> />.
-      + by case: (GWAKEb.state_map{1}.[p{2}])=> /#.
-      by case: (GWAKEb.state_map{1}.[p{2}])=> /#.
-    auto=> /> &1 &2 + + eqsm invl a_in _ _.
-    rewrite -(eqsm (a, i){2}).
-    by case: (GWAKEb.state_map{1}.[(a, i){2}]); smt(get_setE).
-  by auto; smt().
-
-auto=> />.
-split; 1: smt(emptyE).
-move=> a i. 
-apply GWAKE0_undef.
-smt(emptyE).
-qed.
-
-lemma Step1 &m:
-    `|Pr[E_GWAKE(Game1, A).run() @ &m : res] - Pr[E_GWAKE(Game2, A).run() @ &m : res]|
-  = 
-    `|Pr[E_GAEAD(GAEAD0, Red_AEAD(A)).run() @ &m : res] - Pr[E_GAEAD(GAEAD1, Red_AEAD(A)).run() @ &m : res]|.
-proof.
-do! congr.
-+ byequiv => //.
-  proc; inline*.
++ inline*.
   wp.
-  call (:
-        ={psk_map}(Game1, GAEADb)
-     /\ ={state_map}(Game1, Red_AEAD.WAKE_O)
-     /\ (forall a i, Game1_inv Game1.state_map Game1.psk_map a i){1}
-  )=> //.
+  call (: ={state_map, psk_map, bad}(Game4, Red_ROM.WAKE_O)
+       /\ (forall h, h \in Game4.dec_map{1} <=> h \in Red_ROM.WAKE_O.dec_map{2})
+       /\ (forall c ad n, (exists pk, Game4.dec_map{1}.[(pk, ad, c)] = Some n) <=> RO.m{2}.[(ad, c)] = Some n)
+       /\ (forall a b ca cb, ((a, b), msg2_data a b ca, cb) \in Game4.dec_map => ((a, b), msg1_data a b, ca) \in Game4.dec_map){1}
+       /\ (forall a b ca cb caf, ((a, b), msg3_data a b ca cb, caf) \in Game4.dec_map => ((a, b), msg2_data a b ca, cb) \in Game4.dec_map){1}
+  ) => //.
 
-  - conseq (: ={res}
-         /\ ={psk_map}(Game1, GAEADb)
-         /\ ={state_map}(Game1, Red_AEAD.WAKE_O)
-    ) Game1_inv_gen_pskey _ => //.
-    by proc; if; auto.
+  - by proc; sp; if; auto.
 
-  - conseq (: ={res}
-         /\ ={psk_map}(Game1, GAEADb)
-         /\ ={state_map}(Game1, Red_AEAD.WAKE_O)
-    ) Game1_inv_send_msg1 _ => //.
-    proc; inline.
+  - proc; inline*.
     sp; if=> //.
-    by match Some {2} ^match; auto; smt().
-
-  - conseq (: ={res}
-         /\ ={psk_map}(Game1, GAEADb)
-         /\ ={state_map}(Game1, Red_AEAD.WAKE_O)
-    ) Game1_inv_send_msg2 _ => //.
-    proc; inline.
+    seq 1 1 : (#pre /\ ={ca}); 1: by auto.
     sp; if=> //.
-    match Some {2} ^match.
-    + auto; smt().
-    sp; match =.
     + smt().
-    + by auto. 
-    move=> na.
-    by match Some {2} ^match; auto; smt().
-
-  - conseq (: ={res}
-         /\ ={psk_map}(Game1, GAEADb)
-         /\ ={state_map}(Game1, Red_AEAD.WAKE_O)
-    ) Game1_inv_send_msg3 _ => //.
-    proc; inline.
-    sp; if=> //.
-    sp; match = => //. 
-    + smt().
-    move=> st m1.
-    match Some {2} ^match.
-    + auto=> />.
-      move=> &hr smr sml invl ai_in.
-      by case: (invl a{m0} i{m0})=> /#.
-    sp; match =.
-    + by auto=> /#. 
-    + by auto=> /#.
-    move=> nb.
-    match Some {2} ^match.
-    + auto=> /> &1 decl decr smr sml invl ai_in ok _.
-      by case: (invl a{m0} i{m0})=> /#.
+    + rcondt {2} ^if; 1: by auto=> /#. 
+      auto=> />.
+      smt(get_setE).
     by auto=> /#.
-
-  - conseq (: ={res}
-         /\ ={psk_map}(Game1, GAEADb)
-         /\ ={state_map}(Game1, Red_AEAD.WAKE_O)
-    ) Game1_inv_send_fin _ => //.
-    proc; inline.
-    sp; if=> //.
-    sp; match = => //.
-    + smt().
-    move=> st m1 m2.
-    match Some {2} ^match.
-    + auto=> />. 
-      move=> &hr smr sml invl bj_in.
-      by case: (invl b{m0} j{m0})=> /#.
-    by sp; match =; auto=> /#.
-
-  - conseq (: ={res}
-         /\ ={psk_map}(Game1, GAEADb)
-         /\ ={state_map}(Game1, Red_AEAD.WAKE_O)
-    ) Game1_inv_rev_skey _ => //.
-    by sim. 
-
-  - conseq (: ={res}
-         /\ ={psk_map}(Game1, GAEADb)
-         /\ ={state_map}(Game1, Red_AEAD.WAKE_O)
-    ) Game1_inv_test _ => //.
-    by sim. 
   
+   - proc; inline*.
+     sp; if=> //. 
+     match; 1,2: smt().
+     + by auto=> />.
+     move=> nal nar.
+     seq 1 1 : (#pre /\ ={cb}); 1: by auto.
+     sp; if=> //.
+     + smt().
+     + rcondt {2} ^if; 1: by auto=> /#. 
+       auto=> />.
+       smt(get_setE).
+     by auto=> /#.
+
+   - proc; inline*.
+     sp; if=> //. 
+     sp; match = => //.
+     + smt().
+     move=> s m1.
+     sp; match; 1,2: smt().
+     + by auto=> />.
+     move=> nbl nbr.
+     seq 1 1 : (#pre /\ ={caf}); 1: by auto.
+     case (Game4.bad{1}).
+     + rcondf {1} ^if; 1: by auto=> />.
+       rcondf {2} ^if; 1: by auto=> />.
+       by auto=> />.
+     sp; if=> //.
+     + smt().
+     + rcondt {2} ^if; 1: by auto=> /#.
+       rcondf {2} ^if.
+       + auto=> />.
+         smt(mem_set).
+       rcondf {2} ^if.
+       + auto=> />.
+         smt(mem_set).
+       swap {2} ^r1<$ @ ^ok<-.
+       seq 1 1 : (#pre /\ ok{1} = r1{2}); 1: by auto => />.
+       auto=> />.
+       smt(get_setE).
+    by auto=> /#.
+  
+   - proc; inline*.
+     sp; if=> //. 
+     sp; match = => //.
+     + smt().
+     move=> s m1 m2.
+     sp; match; 1,2: smt().
+     + by auto=> />.
+     move=> nokl nokr.
+     rcondf {2} ^if; 1: by auto=> /#.
+     rcondf {2} ^if; 1: by auto=> /#.
+     auto=> />.
+     smt(get_setE).
+  
+   - by sim />.
+   
+   - by sim />.
+
+   auto=> />.
+   smt(emptyE).
+  
+have ll : forall (c : msg_data * ctxt), is_lossless dnonce by move=> _; exact dnonce_ll.
+rewrite equiv [{1} 1 (FullEager.RO_LRO (Red_ROM(A)) ll)].
+inline*.
+wp; call (: 
+  ={state_map, psk_map, bad, dec_map}(Red_ROM.WAKE_O, Game5)
+  /\ (forall a b ca, (forall cb caf, (msg3_data a b ca cb, caf) \notin Game5.prfkey_map{2})
+        => (msg1_data a b, ca) \notin RO.m{1})
+  /\ (forall a b ca cb, (forall caf, (msg3_data a b ca cb, caf) \notin Game5.prfkey_map{2})
+        => (msg2_data a b ca, cb) \notin RO.m{1})
+  /\ (forall a b ca cb caf, (msg3_data a b ca cb, caf) \in Game5.prfkey_map{2} =>
+         exists na nb, Game5.prfkey_map{2}.[(msg3_data a b ca cb, caf)] = Some (na, nb) /\
+                       RO.m{1}.[(msg1_data a b, ca)] = Some na /\
+                       RO.m{1}.[(msg2_data a b ca, cb)] = Some nb)
+  /\ (Game5_inv_full Game5.state_map Game5.dec_map Game5.prfkey_map){2}
+) => //.
+
+- by sim />.
+
+- conseq (: ={res}
+  /\ ={state_map, psk_map, bad, dec_map}(Red_ROM.WAKE_O, Game5)
+  /\ (forall a b ca, (forall cb caf, (msg3_data a b ca cb, caf) \notin Game5.prfkey_map{2})
+        => (msg1_data a b, ca) \notin RO.m{1})
+  /\ (forall a b ca cb, (forall caf, (msg3_data a b ca cb, caf) \notin Game5.prfkey_map{2})
+        => (msg2_data a b ca, cb) \notin RO.m{1})
+  /\ (forall a b ca cb caf, (msg3_data a b ca cb, caf) \in Game5.prfkey_map{2} =>
+         exists na nb, Game5.prfkey_map{2}.[(msg3_data a b ca cb, caf)] = Some (na, nb) /\
+                       RO.m{1}.[(msg1_data a b, ca)] = Some na /\
+                       RO.m{1}.[(msg2_data a b ca, cb)] = Some nb)
+  ) _ Game5_inv_send_msg1 => //.
+  proc; inline*.
+  sp; if=> //.
+  seq 1 1 : (#pre /\ ={ca}); 1: by auto.
+  case (Game5.bad{2}).
+  + rcondf {1} ^if; 1: by auto=> />.
+    rcondf {2} ^if; 1: by auto=> />.
+    auto=> />.
+  sp 1 1; if=> //.
   auto=> />.
-  move=> a i.
-  exact /Game1_undef/emptyE.
-
-byequiv => //.
-proc; inline*.
-wp.
-call (:
-      ={psk_map}(Game2, GAEADb)
-      /\ ={state_map}(Game2, Red_AEAD.WAKE_O)
-      /\ Game2.dec_map{1} = GAEAD1.ctxts{2}
-      /\ (forall a i, Game1_inv Game2.state_map Game2.psk_map a i){1}
-).
-- conseq (: ={res}
-       /\ ={psk_map}(Game2, GAEADb)
-       /\ ={state_map}(Game2, Red_AEAD.WAKE_O)
-       /\ Game2.dec_map{1} = GAEAD1.ctxts{2}
-  ) Game2_inv_gen_pskey _ => //.
-  proc.
-  by if; auto.
 
 - conseq (: ={res}
-       /\ ={psk_map}(Game2, GAEADb)
-       /\ ={state_map}(Game2, Red_AEAD.WAKE_O)
-       /\ Game2.dec_map{1} = GAEAD1.ctxts{2}
-  ) Game2_inv_send_msg1 _ => //.
-  proc; inline.
+  /\ ={state_map, psk_map, bad, dec_map}(Red_ROM.WAKE_O, Game5)
+  /\ (forall a b ca, (forall cb caf, (msg3_data a b ca cb, caf) \notin Game5.prfkey_map{2})
+        => (msg1_data a b, ca) \notin RO.m{1})
+  /\ (forall a b ca cb, (forall caf, (msg3_data a b ca cb, caf) \notin Game5.prfkey_map{2})
+        => (msg2_data a b ca, cb) \notin RO.m{1})
+  /\ (forall a b ca cb caf, (msg3_data a b ca cb, caf) \in Game5.prfkey_map{2} =>
+         exists na nb, Game5.prfkey_map{2}.[(msg3_data a b ca cb, caf)] = Some (na, nb) /\
+                       RO.m{1}.[(msg1_data a b, ca)] = Some na /\
+                       RO.m{1}.[(msg2_data a b ca, cb)] = Some nb)
+  ) _ Game5_inv_send_msg2 => //.
+  proc; inline*.
   sp; if=> //.
-  rcondt{2} ^if; 1: by auto.
-  swap {2} ^c<$ @ ^na<$.
-  by auto.
-
-- conseq (: ={res}
-       /\ ={psk_map}(Game2, GAEADb)
-       /\ ={state_map}(Game2, Red_AEAD.WAKE_O)
-       /\ Game2.dec_map{1} = GAEAD1.ctxts{2}
-  ) Game2_inv_send_msg2 _ => //.
-  proc; inline.
-  sp; if=> //.
-  rcondt {2} 5; 1: by auto.
   sp; match = => //.
-  + by auto.
+  + by auto=> />.
   move=> na.
-  rcondt {2} ^if; 1: by auto.
-  swap {2} ^c0<$ @ ^nb<$.
-  by auto.
+  seq 1 1 : (#pre /\ ={cb}); 1: by auto.
+  case (Game5.bad{2}).
+  + rcondf {1} ^if; 1: by auto=> />.
+    rcondf {2} ^if; 1: by auto=> />.
+    auto=> />.
+  sp 1 1; if=> //.
+  auto=> />.
 
 - conseq (: ={res}
-       /\ ={psk_map}(Game2, GAEADb)
-       /\ ={state_map}(Game2, Red_AEAD.WAKE_O)
-       /\ Game2.dec_map{1} = GAEAD1.ctxts{2}
-  ) Game2_inv_send_msg3 _ => //.
-  proc; inline.
+  /\ ={state_map, psk_map, bad, dec_map}(Red_ROM.WAKE_O, Game5)
+  /\ (forall a b ca, (forall cb caf, (msg3_data a b ca cb, caf) \notin Game5.prfkey_map{2})
+        => (msg1_data a b, ca) \notin RO.m{1})
+  /\ (forall a b ca cb, (forall caf, (msg3_data a b ca cb, caf) \notin Game5.prfkey_map{2})
+        => (msg2_data a b ca, cb) \notin RO.m{1})
+  /\ (forall a b ca cb caf, (msg3_data a b ca cb, caf) \in Game5.prfkey_map{2} =>
+         exists na nb, Game5.prfkey_map{2}.[(msg3_data a b ca cb, caf)] = Some (na, nb) /\
+                       RO.m{1}.[(msg1_data a b, ca)] = Some na /\
+                       RO.m{1}.[(msg2_data a b ca, cb)] = Some nb)
+  ) _ Game5_inv_send_msg3 => //.
+  proc; inline*.
   sp; if=> //.
   sp; match = => //.
   + smt().
-  move=> st m1.
-  rcondt {2} ^if.
-  + auto=> />.
-    move=> &hr smr sml invl ai_in.
-    by case: (invl a{m0} i{m0})=> /#.
-  sp; match =.
-  + by auto.
+  move=> s m1.
+  sp; match = => //.
   + by auto.
   move=> nb.
-  rcondt {2} ^if.
+  seq 1 1 : (#pre /\ ={caf}); 1: by auto.
+  case (Game5.bad{2}).
+  + rcondf {1} ^if; 1: by auto=> />.
+    rcondf {2} ^if; 1: by auto=> />.
+    auto=> />.
+  sp 1 1; if=> //.
+  rcondt {1} ^if.
   + auto=> />.
-    move=> &hr decl decr smr sml invl ai_in ok _.
-    by case: (invl a{m0} i{m0})=> /#.
-  swap {2} ^c0<$ @ ^ok<$.
-  by auto.
+    move=> &hr _ dm _ sm _ inv1 inv2 inv3 invr1 invr2 invr3 invr4 invr5 aiin _ cafnin r _. 
+    have sms : (Game5.state_map.[(a, i)] = Some (role, IPending (b, psk, na, ca) m1)){m0} by smt().
+    case: (invr5 a{m0} i{m0}) ; rewrite sms //=.
+    move=> /> 4!->> _.
+    exact inv1.
+  rcondt {1} ^if.
+  + auto=> />.
+    move=> &hr _ dm _ sm _ inv1 inv2 inv3 invr1 invr2 invr3 invr4 invr5 aiin _ cafnin r _ r1 _. 
+    have sms : (Game5.state_map.[(a, i)] = Some (role, IPending (b, psk, na, ca) m1)){m0} by smt().
+    case: (invr5 a{m0} i{m0}) ; rewrite sms //=.
+    move=> /> 4!->> _.
+    rewrite mem_set /#.
+  outline {2} [3] (na, ok) <@ S.sample. 
+  wp; rewrite equiv [{2} 3 sample_sample2].
+  inline*.
+  auto=> />.
+  move=> &1 &2 _ dm _ sm _ inv1 inv2 inv3 invr1 invr2 invr3 invr4 invr5 aiin _ cafnin r _ r1 _. 
+  rewrite get_set_sameE //=.
+  have smai : (Game5.state_map.[(a, i)] = Some (role, IPending (b, psk, na, ca) m1)){2} by smt().
+  case: (invr5 a{2} i{2}); rewrite smai //=.
+  smt(get_setE).
 
 - conseq (: ={res}
-       /\ ={psk_map}(Game2, GAEADb)
-       /\ ={state_map}(Game2, Red_AEAD.WAKE_O)
-       /\ Game2.dec_map{1} = GAEAD1.ctxts{2}
-  ) Game2_inv_send_fin _ => //.
-  proc; inline.
+  /\ ={state_map, psk_map, bad, dec_map}(Red_ROM.WAKE_O, Game5)
+  /\ (forall a b ca, (forall cb caf, (msg3_data a b ca cb, caf) \notin Game5.prfkey_map{2})
+        => (msg1_data a b, ca) \notin RO.m{1})
+  /\ (forall a b ca cb, (forall caf, (msg3_data a b ca cb, caf) \notin Game5.prfkey_map{2})
+        => (msg2_data a b ca, cb) \notin RO.m{1})
+  /\ (forall a b ca cb caf, (msg3_data a b ca cb, caf) \in Game5.prfkey_map{2} =>
+         exists na nb, Game5.prfkey_map{2}.[(msg3_data a b ca cb, caf)] = Some (na, nb) /\
+                       RO.m{1}.[(msg1_data a b, ca)] = Some na /\
+                       RO.m{1}.[(msg2_data a b ca, cb)] = Some nb)
+  ) _ Game5_inv_send_fin => //.
+- proc; inline*.
   sp; if=> //.
   sp; match = => //.
   + smt().
-  move=> st m1 m2.
-  rcondt {2} 6.
-  + auto=> />.
-    move=> &hr smr sml invl ai_in.
-    by case: (invl b{m0} j{m0})=> /#.
-  sp; match =.
-  + by auto.
+  move=> s m1 m2.
+  sp; match = => //.
   + by auto.
   move=> nok.
-  by auto.
+  rcondf {1} ^if.
+  + auto=> />.
+    move=> &hr dm _ sm _ inv1 inv2 inv3 invr1 invr2 invr3 invr4 invr5 bjin r _.
+    have sms : (Game5.state_map.[(b, j)] = Some (role, RPending (a, psk, na, nb, ca, cb) m1 m2)){m0} by smt().
+    case: (invr5 b{m0} j{m0}) ; rewrite sms //=.
+    smt().
+  rcondf {1} ^if.
+  + auto=> />.
+    move=> &hr dm _ sm _ inv1 inv2 inv3 invr1 invr2 invr3 invr4 invr5 bjin r _ r2 _.
+    have sms : (Game5.state_map.[(b, j)] = Some (role, RPending (a, psk, na, nb, ca, cb) m1 m2)){m0} by smt().
+    case: (invr5 b{m0} j{m0}) ; rewrite sms //=.
+    smt().
+  auto=> />.
+  smt().
 
 - conseq (: ={res}
-       /\ ={psk_map}(Game2, GAEADb)
-       /\ ={state_map}(Game2, Red_AEAD.WAKE_O)
-       /\ Game2.dec_map{1} = GAEAD1.ctxts{2}
-  ) Game2_inv_rev_skey _ => //.
-  by sim.
+  /\ ={state_map, psk_map, bad, dec_map}(Red_ROM.WAKE_O, Game5)
+  /\ (forall a b ca, (forall cb caf, (msg3_data a b ca cb, caf) \notin Game5.prfkey_map{2})
+        => (msg1_data a b, ca) \notin RO.m{1})
+  /\ (forall a b ca cb, (forall caf, (msg3_data a b ca cb, caf) \notin Game5.prfkey_map{2})
+        => (msg2_data a b ca, cb) \notin RO.m{1})
+  /\ (forall a b ca cb caf, (msg3_data a b ca cb, caf) \in Game5.prfkey_map{2} =>
+         exists na nb, Game5.prfkey_map{2}.[(msg3_data a b ca cb, caf)] = Some (na, nb) /\
+                       RO.m{1}.[(msg1_data a b, ca)] = Some na /\
+                       RO.m{1}.[(msg2_data a b ca, cb)] = Some nb)
+  ) _ Game5_inv_rev_skey => //.
+  by sim />.
 
 - conseq (: ={res}
-       /\ ={psk_map}(Game2, GAEADb)
-       /\ ={state_map}(Game2, Red_AEAD.WAKE_O)
-       /\ Game2.dec_map{1} = GAEAD1.ctxts{2}
-  ) Game2_inv_test _ => //.
-  by sim.
+  /\ ={state_map, psk_map, bad, dec_map}(Red_ROM.WAKE_O, Game5)
+  /\ (forall a b ca, (forall cb caf, (msg3_data a b ca cb, caf) \notin Game5.prfkey_map{2})
+        => (msg1_data a b, ca) \notin RO.m{1})
+  /\ (forall a b ca cb, (forall caf, (msg3_data a b ca cb, caf) \notin Game5.prfkey_map{2})
+        => (msg2_data a b ca, cb) \notin RO.m{1})
+  /\ (forall a b ca cb caf, (msg3_data a b ca cb, caf) \in Game5.prfkey_map{2} =>
+         exists na nb, Game5.prfkey_map{2}.[(msg3_data a b ca cb, caf)] = Some (na, nb) /\
+                       RO.m{1}.[(msg1_data a b, ca)] = Some na /\
+                       RO.m{1}.[(msg2_data a b ca, cb)] = Some nb)
+  ) _ Game5_inv_test => //.
+  by sim />.
 
-auto=> />.
-move=> a i.
-exact /Game1_undef/emptyE.
+auto => />.
+smt(emptyE Game5_undef).
 qed.
